\documentclass{article}
\usepackage{amsmath}
\usepackage{amsthm}
\usepackage{amssymb}
\usepackage{enumerate}
\usepackage{tikz}
\usepackage{graphicx}

\begin{document}
  \title{Exercise 15.6}
  \author{Wang Yue from CS Elite Class}
  \maketitle

  \subsection*{6. }

  Let $f(x, y) = 4 - x^2 - y^2$ and $D = \{ (x, y) | x^2 + y^2 \leq 4\}$, then

  $f_x(x, y) = -2x, f_y(x, y) = -2y$

  $$\begin{aligned}
    \iint_D\sqrt{[f_x(x, y)]^2 + [f_y(x, y)]^2 + 1} dA &= \iint_D \sqrt{4x^2 + 4y^2 + 1} dA \\
    &= \int_0^{2\pi} \int_0^2 \sqrt{4r^2 + 1}r dr d\theta \\
    &= \int_0^{2\pi} \int_0^2 \frac 1 8 \sqrt{4r^2 + 1}d(4r^2 + 1) d\theta \\
    &= \int_0^{2\pi} \frac 1 8\times \frac 2 3 (4r^2 + 1)^{\frac 3 2}\biggl|_0^2 d\theta \\
    &= \int_0^{2\pi} \frac{1}{12} (17^{\frac 3 2} - 1) d\theta \\
    &= \frac{(17^{\frac 3 2} - 1)\pi}{6}
  \end{aligned}$$

  \subsection*{11. }

  Let $f(x, y) = \sqrt{a^2-x^2-y^2}$ and $D = \{ (x, y) | x^2 + y^2 \leq ax \}$, then

  $$f_x(x, y) = \frac{-x}{\sqrt{a^2-x^2-y^2}}, f_y(x, y) = \frac{-y}{\sqrt{a^2-x^2-y^2}}$$

  $$\begin{aligned}
    \iint_D \sqrt{[f_x(x, y)]^2 + [f_y(x, y)]^2 + 1} dA &= \iint_D \sqrt{\frac{x^2+y^2+a^2-x^2-y^2}{a^2-x^2-y^2}} dA \\
    &= \int_{-\pi}^{\pi} \int_0^{a\cos \theta} \sqrt{\frac{a^2}{a^2-r^2}} r dr d\theta \\
    &= a\int_{-\pi}^{\pi} \int_0^{a\cos \theta} (-\frac 1 2) (a^2-r^2)^{-\frac 1 2} d(a^2-r^2) d\theta \\
    &= a\int_{-\pi}^{\pi} - (a^2-r^2)^{\frac 1 2}\biggl|_{r=0}^{r=a\cos \theta} d\theta \\
    &= a\int_{-\pi}^{\pi} a(1 - \sin \theta) d\theta \\
    &= a^2(\theta + \cos \theta)\biggl|_{-\pi}^{\pi} \\
    &= a^2(2\pi - 2)
  \end{aligned}$$

  \subsection*{12. }

  $\because \left\{ \begin{array}{ll}  x^2+y^2+z^2=4z \\ z = x^2 + y^2  \end{array}\right. \implies x^2 + y^2 = 3$

  $\therefore D = \{ (x, y) | x^2 + y^2 = 3 \}$

  $\because x^2 + y^2 + z^2 = 4z$

  $\therefore z^2 - 4z + 4 = 4 - x^2 - y^2 = (z-2)^2$

  $\therefore z - 2 = \sqrt{4 - x^2 - y^2}, z = \sqrt{4 - x^2 - y^2} + 2$

  $$\begin{aligned}
    \iint_D \sqrt{1 + (\frac{\partial z}{\partial x})^2 + (\frac{\partial z}{\partial y})^2} dA &=  \int_0^{2\pi} \int_0^{\sqrt 3} \sqrt{1 + (\frac{-r\cos \theta}{\sqrt{4-r^2}})^2 + (\frac{-r\sin \theta}{\sqrt{4-r^2}})^2} r dr d\theta \\
    &= \int_0^{2\pi} \int_0^{\sqrt 3} \sqrt{\frac{4-r^2+r^2}{4-r^2}} r dr d\theta \\
    &= \int_0^{2\pi} \int_0^{\sqrt 3} 2\sqrt{\frac{1}{4-r^2}}r dr d\theta \\
    &= -\int_0^{2\pi} \int_0^{\sqrt 3} (4-r^2)^{-\frac 1 2} d(4-r^2) dr d\theta \\
    &= -\int_0^{2\pi}  2(4-r^2)^{\frac 1 2}\biggl|_{r=0}^{r=\sqrt 3} d\theta \\
    &= -\int_0^{2\pi} 2(1-2)d\theta \\
    &= 4\pi
  \end{aligned}$$

  \subsection*{22. }

  The area of the top half of the sphere is
  $$\lim_{t \to a^-} \iint_D \sqrt{1 + (\frac{\partial z}{\partial x})^2 + (\frac{\partial z}{\partial y})^2} dA$$

  where $\frac{\partial z}{\partial x} = \frac{-x}{\sqrt{t^2 - x^2 - y^2}}, \frac{\partial z}{\partial y} = \frac{-y}{\sqrt{t^2 - x^2 - y^2}}, D = \{ (x, y) | x^2 + y^2 \leq t^2 \}$

  $$\begin{aligned}
    \lim_{t \to a^-} \iint_D \sqrt{1 + (\frac{\partial z}{\partial x})^2 + (\frac{\partial z}{\partial y})^2} dA &= \lim_{t \to a^-} \int_0^{2\pi} \int_0^t \sqrt{1 + (\frac{-r\cos \theta}{\sqrt{t^2 - r^2}})^2 + (\frac{-r\sin \theta}{\sqrt{t^2-r^2}})^2} r dr d\theta \\
    &= \lim_{t \to a^-} \int_0^{2\pi} \int_0^t \sqrt{\frac{t^2-r^2 + r^2}{t^2-r^2}} r dr d\theta \\
    &= \lim_{t \to a^-} \int_0^{2\pi} (-\frac 1 2) t (t^2 - r^2)^{-\frac 1 2} d(t^2 - r^2) d\theta \\
    &= \lim_{t \to a^-} \int_0^{2\pi} -t(t^2-r^2)^{\frac 1 2}\biggl|_{r=0}^{r=t} d\theta \\
    &= \lim_{t \to a^-} \int_0^{2\pi} t^2 d\theta \\
    &= \lim_{t \to a^-} 2\pi t^2 \\
    &= 2\pi a^2
  \end{aligned}$$

  $\therefore$ the area of a sphere of radius $r$ is $2 \times 2\pi a^2 = 4\pi a^2$

  \subsection*{23. }

  $D = \{ (x, y) | x^2 + y^2 = \leq 25 \}$

  $$\begin{aligned}
    \iint_D \sqrt{1 + (\frac{\partial z}{\partial x})^2 + (\frac{\partial z}{\partial y})^2} dA &= \iint_D \sqrt{1 + (\frac{\partial y}{\partial x})^2 + (\frac{\partial y}{\partial z})^2} dA \\
    &= \iint_D \sqrt{1 + (2x)^2 + (2z)^2} dx dz \\
    &= \int_0^{2\pi} \int_0^5 \sqrt{1 + 4r^2} r dr d\theta \\
    &= \frac 1 8 \int_0^{2\pi} \int_0^5 \sqrt{1 + 4r^2} d(1 + 4r^2) d\theta \\
    &= \frac 1 8 \int_0^{2\pi} \frac 2 3 (1 + 4r^2)^{\frac 3 2}\biggl|_{r=0}^{r=5} d\theta \\
    &= \frac {1}{12} \int_0^{2\pi} (101)^{\frac 3 2} - 1 d\theta \\
    &= \frac{101^{\frac 3 2} - 1}{6} \pi
  \end{aligned}$$

  \subsection*{24. }

  Solving $\left\{ \begin{array}{ll} x^2+z^2=1 \\ y^2+z^2=1 \end{array} \right.$, intersection points are as follows:

  $(1, -1, 0), (1, 1, 0), (-1, 1, 0), (-1, -1, 0), (0, 0, 1), (0, 0, -1)$

  $V = 8V_1$

  $$\begin{aligned}
    V_1 &= \int_0^1 dz \int_0^{\sqrt{1-z^2}}dx \int_0^{\sqrt{1-z^2}} dy \\
    &= \int_0^1 (\sqrt{1-z^2})^2 dz \\
    &= (z - \frac 1 3 z^3)\biggl|_0^1 \\
    &= 1 - \frac 1 3 - 0 = \frac 2 3
  \end{aligned}$$

  $$\therefore V = 8V_1 = \frac{16}{3}$$
  
\end{document}