\documentclass{article}
\usepackage{amsmath}
\usepackage{amsthm}
\usepackage{amssymb}
\usepackage{enumerate}
\usepackage{tikz}
\usepackage{graphicx}

\begin{document}
  \title{Exercise 9.5}
  \author{Wang Yue from CS Elite Class}
  \maketitle

  \subsection*{10. $ y' + y = \sin e^x $}

  Integrating factor: $e^{\int 1 dx} = e^x$

  $$e^x y' + e^x y = \frac{d}{dx} (ye^x) = e^x \sin e^x$$
  
  $$\int \frac{d}{dx} (ye^x) dx = \int \sin e^x dx$$

  $$ye^x = -\cos e^x + C$$

  $$y = -\cos x + Ce^{-x}$$

  where $C$ is an arbitrary constant

  \subsection*{11. $ \sin x \frac{dy}{dx} + (\cos x)y = \sin(x^2) $}

  $$\int \frac{d}{dx} (y \sin x) dx = \int \sin(x^2) dx$$

  $$y = \frac{\int \sin(x^2) dx + C}{ \sin x}$$

  where $\int \sin(x^2) dx$ is an integral that cannot be solved directly, $C$ is an arbitrary constant.

  \subsection*{14. $ t \ln t \frac{dr}{dt} + r = te^t $}

  $$\frac{dr}{dt} + \frac{1}{t\ln t} r = \frac{e^t}{\ln t}$$

  Integrating factor: $ e^{\int \frac{1}{t\ln t} dt} = e^{\int \frac{1}{\ln t} d\ln t} = e^{\ln (\ln t)} = \ln t$

  $$\ln t \frac{dr}{dt} + \frac{1}{t} r = \frac{d}{dx} (r \ln t) = e^t$$

  $$r \ln t = \int e^t dt = e^t + C$$

  $$\therefore r\ln t = e^t + C$$

  where $C$ is an arbitrary constant

  \subsection*{15. }

  $$x^2 y' + 2xy = \frac{d}{dx} (x^2y) = \ln x$$

  $$x^2y = \int \ln x dx = x\ln x - x + C$$

  Since $2 = 0 - 1 + C$, $C = 3$

  $$\therefore x^2y = x\ln x - x + 3$$

  \subsection*{16. }

  $$\frac{d}{dt} (t^3 y) = \cos t $$

  $$t^3y = \int \cos t dt = \sin t + C$$

  Since $\pi^3\times 0 = \sin \pi + C$, $C = 0$

  $$\therefore t^3 y = \sin t$$

  \subsection*{23. }

  Let $u = y^{1-n}$, then

  $$\frac{du}{dx} = \frac{du}{dy} \frac{dy}{dx} = (1-n)y^{-n} \frac{dy}{dx}$$

  Multiplied by $(1-n)y^{-n}$ on the both sides, we get

  $$(1-n)y^{-n} \frac{dy}{dx} + (1-n)y^{1-n}P(x) =(1-n) Q(x)$$
  
  which is equivalent to

  $$\frac{du}{dx} + (1-n)P(x) u = (1-n)Q(x)$$

  \subsection*{25. }

  Let $u = y^{1-3} = y^{-2}$

  Multiplied by $(1-3) y^{-3}$ on the both sides, we get

  $$(-2)y^{-3} y' + (-2) \frac{2}{x} y^{-2} = \frac{-2}{x^2}$$

  which is equivalent to

  $$\frac{du}{dx} - \frac{4}{x} u = \frac{-2}{x^2}$$

  Integrating factor: $ e^{\int -\frac{4}{x} dx} = e^{-4\ln x} = x^{-4} $

  $$x^{-4} \frac{du}{dx} - 4x^{-5} u = \frac{d}{dx}(x^{-4} u) = -2x^{-6}$$

  $$x^{-4} u = \int -2x^{-6} dx + C = \frac 2 5 \int -5x^{-6} dx + C = \frac 2 5 x^{-5} + C$$

  $$\therefore u = \frac 2 5 x^{-1} + Cx^4$$

  where $C$ is an arbitrary constant

  \subsection*{26. }

  Let $ u = y' $, then

  $$x \frac{du}{dx} + 2u = 12x^2 \iff \frac{du}{dx} + \frac 2 x u = 12x$$

  Integrating factor: $e^{\int \frac 2 x dx} = x^2$

  $$x^2 \frac{du}{dx} + 2x u = \frac{d}{dx}(x^2u) = 12x^3$$

  $$x^2 u = \int 12x^3 dx = 3x^4 + C$$

  $$ u = 3x^2 + \frac{C}{x^2}$$

  where $C$ is an arbitrary constant

\end{document}
