\documentclass{article}
\usepackage{amsmath}
\usepackage{amsthm}
\usepackage{amssymb}
\usepackage{enumerate}
\usepackage{tikz}
\usepackage{graphicx}

\begin{document}
  \title{Exercise 16.7}
  \author{Wang Yue from CS Elite Class}
  \maketitle

  \subsection*{4. }

  $$\begin{aligned}
    \iint_S f(x, y, z) dS &= \iint_S g(\sqrt{x^2+y^2+z^2}) dS  \\
    &= \iint_S g(2) dS \\
    &= -5 \iint_S dS = -5 \times 16 \pi = -80\pi 
  \end{aligned}$$

  \subsection*{6. }

  $$\overrightarrow{r_u} = \langle \cos v, \sin v, 1 \rangle$$

  $$\overrightarrow{r_v} = \langle -u\sin v, u\cos v, 0 \rangle$$

  $$\overrightarrow{r_u} \times \overrightarrow{r_v} = \langle -u\cos v, -u\sin v, u \rangle$$

  $$|\overrightarrow{r_u} \times \overrightarrow{r_v}| = \sqrt{u^2 + u^2} = \sqrt 2 u$$

  $$\begin{aligned}
    \iint_S xyz dS &= \int_0^1 \int_0^{\frac \pi 2} \sqrt 2 u^4 \sin v \cos v dv du \\
    &= \sqrt 2 \int_0^1 \int_0^{\frac \pi 2} u^4 \sin v d\sin v du \\
    &= \sqrt 2 \int_0^1 u^4 (\frac{\sin^2 v}{2})\biggl|_0^{\frac \pi 2} du \\
    &= \frac{\sqrt 2}{2} \int_0^1 u^4 du \\
    &= \frac{\sqrt 2}{2} \times (\frac{u^5}{5})\biggl|_0^1 \\
    &= \frac{\sqrt 2}{10}
  \end{aligned}$$

  \subsection*{10. }

  $\because z = 4 - 2x - 2y$

  $\therefore \frac{\partial z}{\partial x} = -2, \frac{\partial z}{\partial y} = -2$

  $$\begin{aligned}
    \iint_S xz dS &= \iint_{D_{xy}} x(4-2x-2y) \sqrt{(-2)^2 + (-2)^2 + 1} dA \\
     &= \int_0^2 \int_0^{2-x} 3x(4-2x-2y) dy dx \\
     &= \int_0^2 (12xy - 6x^2y - 3xy^2)\biggl|_0^{2-x} dx \\
     &= \int_0^2 [12x(2-x) - 6x^2(2-x) - 3x(2-x)^2] dx \\
     &= \int_0^2 (3x^3 - 12x^2 + 12x) dx \\
     &= (\frac{3x^4}{4} - 4x^3 + 6x^2)\biggl|_0^2  \\
     &= 12 - 4 \times 8 + 6 \times 4 = 4
  \end{aligned}$$

  \subsection*{14. }

  $\because x = y + 2z^2$

  $\therefore \frac{\partial x}{\partial y} = 1, \frac{\partial x}{\partial z} = 4z$

  $$\begin{aligned}
    \iint_S z dS &= \iint_{D_{yz}} z \sqrt{1^2 + (4z)^2 + 1} dA\\
    &= \int_0^1 \int_0^1 z \sqrt{16z^2 + 2} dy dz \\
    &= \int_0^1 z \sqrt{16z^2 + 2} dz \\
    &= \frac{1}{32} \int_0^1 \sqrt{16z^2+2} d(16z^2 + 2) \\
    &= \frac{1}{32} \times \frac 2 3 (16z^2 + 2)^{\frac 3 2}\biggl|_0^1 \\
    &= \frac{1}{48} (162\sqrt 2 - 2\sqrt 2) \\
    &= \frac{10\sqrt 2}{3}
  \end{aligned}$$

  \subsection*{15. }

  $$\begin{aligned}
    \iint_S y dS &= \iint_D (x^2+z^2) \sqrt{4x^2+4z^2+1} dA \\
    &= \int_0^{2\pi} \int_0^2 r^2 \sqrt{4r^2 + 1} r dr d\theta \\
  \end{aligned}$$

  Let $t = 4r^2 + 1$, $r^2 = \frac{t-1}{4}$ then $dt = 8r dr$, so

  $$\begin{aligned}
    \int_0^{2\pi} \int_0^2 r^2 \sqrt{4r^2 + 1} r dr d\theta &= \int_0^{2\pi} \int_0^2 \frac{t-1}{4} \sqrt{t} \frac 1 8 dt d\theta \\
    &= \frac{1}{32} \int_0^{2\pi} \int_0^2 (t^{\frac 3 2} - t^{\frac 1 2}) dt d\theta \\
    &= \frac{1}{32} \int_0^{2\pi} (\frac 2 5 t^{\frac 5 2} - \frac 2 3 t^{\frac 3 2})\biggl|_0^2 d\theta \\
    &= \frac{\pi}{8} (\frac{4\sqrt 2}{5} - \frac{2\sqrt 2}{3})
  \end{aligned}$$


  \subsection*{18. }

  % Let $x = x, y = 3 \cos \theta, z = 3 \sin \theta$, then

  % $$\overrightarrow{r_x} = \langle 1, 0, 0 \rangle$$

  % $$\overrightarrow{r_\theta} = \langle 0, -3\sin \theta, 3 \cos \theta \rangle$$

  % $$|\overrightarrow{r_x} \times \overrightarrow{r_\theta}| = |\langle 0, -3\cos \theta, -3\sin \theta| = 3$$

  % Since $S_1$ lies in plane $x = 0$, $\iint_{S_1} xz dS = 0$

  % $$\begin{aligned}
  %   \iint_{S_2} xz dS &= \int_0^{2\pi} \int_0^{5 - 3 \cos \theta} 9x\sin \theta dx d\theta \\
  %   &= 9\int_0^{2\pi} \sin \theta \int_0^{5-3\cos \theta} x dx d\theta \\
  %   &= 9\int_0^{2\pi} \sin \theta (\frac{x^2}{2})\biggl|_0^{5-3\cos \theta} d\theta \\
  %   &= \frac 9 2 \int_0^{2\pi} (25\sin \theta + 9\sin \theta \cos^2 \theta - 30 \sin \theta \cos \theta) d\theta \\
  %   &= \frac 9 2 (-25\cos \theta)\biggl|_0^{2\pi} + (-3 \cos^3 \theta)\biggl|_0^{2\pi} - (15\sin^2 \theta)\biggl|_0^{2\pi} \\
  %   &= 0
  % \end{aligned}$$

  Let the surface of the cylinder on $yOz$ plane, on the side face, on $x + y = 5$ be $S_1$, $S_2$, $S_3$, respectively.

  $$\iint_{S_1} xz dS = 0$$

  Let $y = 3 \cos \theta, z = 3 \sin \theta, x = x$, then

  $$\overrightarrow{r_\theta} = \langle 0, -3\sin \theta, 3\cos \theta \rangle, \overrightarrow{r_x} = \langle 1, 0, 0 \rangle$$

  $$\begin{aligned}
    \iint_{S_2} xz dS &= \iint_{D} xz |\overrightarrow{r_\theta} \times \overrightarrow{r_x}| dA \\
                     &= 3\iint_D xz dA \\
                     &= 3\int_0^{2\pi} \int_{0}^{5-3\cos \theta} 3x \sin \theta dx d\theta \\
                     &= 9\int_0^{2\pi} \sin \theta (\frac{x^2}{2})\biggl|_0^{5-3\cos \theta} d\theta \\
                     &= \frac{9}{2} \int_0^{2\pi}  (25 \sin \theta + 9 \sin \theta \cos^2 \theta - 30 \sin \theta \cos \theta) d\theta \\
                     &= 0
  \end{aligned}

  $$\begin{aligned}
    \iint_{S_3} xz dS &= \iint_D (5-y)z \sqrt{1 + (\frac{\partial x}{\partial y})^2 + (\frac{\partial x}{\partial z})^2} dA \\
                      &= \int_0^{2\pi} \int_0^3 (5-r \cos \theta)(r \sin \theta) \sqrt{1 + 1 + 0} r dr d\theta \\
                      &= \sqrt 2 \int_0^{2\pi}  \sin \theta \int_0^3 (5r^2-r^3\cos \theta) dr d\theta \\
                     &= \sqrt 2 \int_0^{2\pi} (\frac{5}{3}r^3 - \frac{r^4 \cos \theta}{4})\biggl|_0^3 d\theta \\
                     &= \sqrt 2 \int_0^{2\pi} (45 - \frac{81}{4}\cos \theta) d\theta \\
                     &= \sqrt 2(45\theta - \frac{81}{4} \sin \theta)\biggl|_0^{2\pi} \\
                     &= 90\sqrt 2 \pi
  \end{aligned}

  $$\therefore \iint_S xz dS = \iint_{S_1} xz dS + \iint_{S_2} xz dS + \iint_{S_3} xz dS = 90\sqrt 2 \pi $$

  \subsection*{24. }

  $$\overrightaarrow{F(x, y, z) = \langle -x, -y, z^3 \rangle$$

    $$z = \sqrt{x^2 + y^2}, (x, y) \in [1, 9]$$

    $$\frac{\partial z}{\partial x} = \frac{x}{\sqrt{x^2+y^2}}, \frac{\partial z}{\partial y} = \frac{y}{\sqrt{x^2+y^2}}$$

    $$\overrightarrow{n} = \frac{\frac{\partial z}{\partial x}\overrightarrow i + \frac{\partial z}{\partial y} \overrightarrow j - \overrightarrow k}{\sqrt{1 + (\frac{\partial z}{\partial x})^2 + (\frac{\partial z}{\partial y})^2}} = \frac{\frac{x}{\sqrt{x^2+y^2}} \overrightarrow{i} + \frac{y}{\sqrt{x^2+y^2}} \overrightarrow{j} - \overrightarrow{k}}{\sqrt{1 + (\frac{\partial z}{\partial x})^2 + (\frac{\partial z}{\partial y})^2}}$$

  $$\begin{aligned}
    \iint_S \overrightarrow{F} \cdot \overrightarrow{n} dS &= \iint_D \frac{-\frac{x^2}{\sqrt{x^2+y^2}} -\frac{y^2}{\sqrt{x^2+y^2}} -z^3}{\sqrt{1 + (\frac{\partial z}{\partial x})^2 + (\frac{\partial z}{\partial y})^2}} \sqrt{1 + (\frac{\partial z}{\partial x})^2 + (\frac{\partial z}{\partial y})^2} dA \\
                                                           &= \iint_D -\sqrt{x^2+y^2} - (x^2+y^2) dA \\
                                                           &= \int_0^{2\pi} \int_1^3 (-r-r^2)r dr d\theta \\
                                                           &= \int_0^{2\pi} (-\frac{r^3}{3} - \frac{r^4}{4})\biggl|_1^{3} d\theta \\
                                                           &= \int_0^{2\pi} (-9 - \frac{81}{4} + \frac{1}{3} + \frac{1}{4})a d\theta \\
                                                           &= 2\pi \times (-9 - 20 + \frac{1}{3}) \\
                                                           &= -\frac{172\pi}{3}
  \end{aligned}
  $$

  \subsection*{25. }

  $$\overrightarrow{F}(x, y, z) = \langle x, -z,  y \rangle$$

  Let $x = \sin \varphi \cos \theta, y = \sin \varphi \sin \theta, z = \cos \varphi$

  $$\overrightarrow{r_\varphi} = \langle \cos \varphi \cos \theta, \cos \varphi \sin \theta, -\sin \varphi \rangle, \overrightarrow{r_\theta} = \langle -\sin \varphi \sin \theta, \sin \varphi \cos \theta, 0 \rangle$$

  $$\overrightarrow{n} = \frac{\overrightarrow{r_\varphi} \times \overrightarrow{r_\theta}}{|\overrightarrow{r_\varphi} \times \overrightarrow{r_\theta}|} = \frac{\langle \sin^2 \varphi \cos \theta, \sin^2 \varphi \sin \theta, \sin \varphi \cos \varphi \rangle}{|\overrightarrow{r_\varphi} \times \overrightarrow{r_\theta}|}$$

  $$\begin{aligned}
    \iint_S \overrightarrow{F} \cdot \overrightarrow{n} dS &= \iint_D (\sin^3 \varphi  \cos^2 \theta+ \sin^3 \varphi \sin^2 \theta+ \sin^2 \varphi \cos^2 \varphi) dA \\
                                                           &= \int_0^{\frac{\pi}{2}} \int_0^{\frac{\pi}{2}} (\sin^3 \varphi + \sin^2 \varphi \cos^2 \varphi) d\varphi d\theta \\
                                                           &= \frac{\pi}{2} \int_0^{2\pi} (\cos^2 \varphi - 1) d\cos \varphi + \frac{\pi}{8} \int_0^{\frac{\pi}{2}} \sin^2 (2x) dx \\
                                                           &= \frac{\pi}{2} [\frac{\cos^3x}{3} - \varphi]\biggl|_0^{2\pi} + \frac{\pi}{8} \int_0^{\frac{\pi}{2}} \frac{1-\cos 4x}{2} dx \\
                                                           &= -\pi^2 + \frac{\pi}{16} (\frac{\pi}{2} - \frac{\sin 4x}{4}\biggl|_0^{\frac{\pi}{2}}) \\
                                                           &= -\pi^2 + \frac{\pi^2}{32} = -\frac{31}{32}\pi^2
  \end{aligned}
  $$

  \subsection*{30. }

  $$\overrightarrow{F} = \langle x, y, 5 \rangle$$

  Let the surface of the cylinder in plane $y = 0$, in side face, in $x + y = 2$ be $S_1$, $S_2$, $S_3$, respectively.

  For surface $S_1$, $\overrightarrow{n} = \langle 0, 1, 0 \rangle$

  $$\iint_{S_1} \overrightarrow{F} \cdot \overrightarrow{n} dS = \iint_{S_1} y dS = 0$$

  For surface $S_2$, let $x = \cos \theta, z = \sin \theta, y = y$, then $\overrightarrow{n} = \langle \cos \theta, 0, \sin \theta \rangle$

  $$\begin{aligned}
    \iint_{S_2} \overrightarrow{F} \cdot \overrightarrow{n} dS &= \int_0^{2\pi} \int_0^{2-\cos \theta} (\cos^2 \theta + 5\sin \theta) dy d\theta  \\
                                                               &= \int_0^{2\pi} (5\sin \theta + \cos^2 \theta)(2- \cos \theta) d\theta \\
                                                               &= \int_0^{2\pi} 10\sin\theta - 5\sin \theta \cos \theta + 2\cos^2 \theta - \cos^3 \theta d\theta \\
                                                               &= 2\pi
  \end{aligned}
  $$

  For surface $S_3$, let $x = u \cos \theta, y = 2 - u \cos \theta, z = u \sin \theta$

  $$\overrightarrow{r_u} = \langle \cos \theta, -\cos \theta, \sin \theta \rangle, \overrightarrow{r_\theta} = \langle -u\sin \theta, u \sin \theta, u \cos \theta \rangle$$

  $$\overrightaarrow{n} = -\frac{\overrightarrow{r_u} \times \overrightarrow{r_\theta}}{|\overrightarrow{r_u} \times \overrightarrow{r_\theta}|} = \frac{\langle u, u, 0 \rangle}{|\overrightarrow{r_u} \times \overrightarrow{r_\theta}|}$$

  $$\begin{aligned}
    \iint_{S_3} \overrightarrow{F} \cdot \overrightarrow{n} dS &= \iint_D (u^2 \cos \theta + 2u - u^2 \cos \theta) dA \\
                                                               &= 2\iint_D u dA \\
                                                               &=  \int_0^{2\pi} \int_0^1 2u du d\theta \\
                                                               &= \int_0^{2\pi} (u^2)\biggl|_0^1 d\theta \\
                                                               &= 2\pi
\end{aligned}$$

$\therefore$ the general solution is

$$y = 0 + 2\pi + 2\pi = 4\pi$$

  \subsection*{31. }

  Let $x = v, y = \cos u, z = \sin u, u \in [0, \pi], v \in [0, 2]$

  $$\overrightarrow{F} = \langle v^2, \cos^2 u, \sin^2 u \rangle$$

  $$\overrightarrow{r_u} = \langle 0, -\sin u, \cos u \rangle, \overrightarrow{r_v} = \langle 1, 0, 0 \rangle$$

  $$\overrightarrow{n} = \frac{\overrightarrow{r_u} \times \overrightarrow{r_v}}{|\overrightarrow{r_u} \times \overrightarrow{r_v}|} = \frac{\langle 0, \cos u, \sin u \rangle}{|\overrightarrow{r_u} \times \overrightarrow{r_v}|}$$

  $$\begin{aligned}
    \iint_S \overrightarrow{F} \cdot \overrightarrow{n} dS &= \iint_D \cos^3 u + \sin^2 u \cos u dA \\
                                                           &= \int_0^\pi \int_0^2 \cos u dv du \\
                                                           &= \int_0^\pi 2\cos u du \\
                                                           &= 0
  \end{aligned} $$

  \subsection*{37. }

  $$\overrightarrow{n} = \frac{\langle \frac{\partial h}{\partial x}, -1, \frac{\partial h}{\partial z} \rangle}{|\overrightarrow{\langle \frac{\partial h}{\partial x}, -1, \frac{\partial h}{\partial z} \rangle}|}$$

  Let $\overrightarrow{F} = \langle P, Q, R \rangle$, then

  $$\iint_S \overrightarrow{F} \cdot d\overrightarrow{S} = \iint_D (P \frac{\partial h}{\partial x} - Q + R \frac{\partial h}{\partial z}) dA$$

  \subsection*{38. }

  $$\overrightarrow{n} = \frac{\langle 1, -\frac{\partial k}{\partial y}, -\frac{\partial k}{\partial z} \rangle}{|\langle 1, -\frac{\partial k}{\partial y}, -\frac{\partial k}{\partial z} \rangle|}$$
  
  Let $\overrightarrow{F} = \langle P, Q, R \rangle$, then

  $$\iint_S \overrightarrow{F} \cdot d\overrightarrow{S} = \iint_D (P - Q \frac{\partial k}{\partial y} - R \frac{\partial k}{\partial z}) dA$$

\end{document}
