\documentclass{article}
\usepackage{amsmath}
\usepackage{amsthm}
\usepackage{amssymb}
\usepackage{enumerate}
\usepackage{tikz}
\usepackage{graphicx}

\begin{document}
  \title{Exercise 17.2}
  \author{Wang Yue from CS Elite Class}
  \maketitle

  \subsection*{6. }
  
  The auxiliary equation is $\lambda^2 - 4\lambda + 4 = 0$ with a double root $2$.

  For the equation $y'' - 4y' + 4y = 0$, $y_c = C_1 e^{2x} + C_2 x e^{2x}$

  For the equation $y'' - 4y' + 4y = xe^{0x}$, let $y_{p_1}(x) = Ax + B$.

  Then $y_{p_1}'(x) = A$, $y_{p_1}''(x) = 0$, so

  $$-4A + 4(Ax + B) = 4Ax + 4B - 4A =  1x + 0$$

  $\therefore A = B = \frac 1 4$

  $\therefore y_{p_1}(x) = \frac 1 4 x + \frac 1 4$

  For the equation $y'' - 4y' + 4y = -\sin x$, let $y_{p_2}(x) = C \sin x + D \cos x$.

  Then $y_{p_2}'(x) = C \cos x - D \sin x, y_{p_2}''(x) = -C \sin x - D \cos x$, so

  $$(-C\sin x - D \cos x) - 4(C \cos x - D \sin x) + 4(C \sin x + D \cos x) = -\sin x$$

  $$(4D+3C) \sin x + (-4C+3D) \cos x = -1\sin x + 0\cos x$$

  Finally, $C = -\frac{3}{25}, D = \frac 4 3 D = -\frac{4}{25}$

  $\therefore y_{p_2}(x) = -\frac{3}{25} \sin x - \frac{4}{25} \cos x$

  $\therefore$ the general solution is

  $$\begin{aligned}
    y &= y_c + y_{p_1} + y_{p_2} \\
      &= C_1 e^{2x} + C_2 xe^{2x} + \frac 1 4 x + \frac 1 4 - \frac{3}{25} \sin x - \frac{4}{25} \cos x
  \end{aligned}$$

  where $C_1$ and $C_2$ are arbitrary constants.

  \subsection*{7. }

  The auxiliary equation $\lambda^2 + 1 = 0$, with complex roots $\lambda = \pm i$.

  For the equation $y'' + y = 0$, $y_c = C_1 \cos x + C_2 \sin x$

  For the equation $y'' + y = e^x$, let $y_{p_1}(x) = Ae^x$.

  Then $y_{p_1}'(x) = y_{p_1}''(x) = Ae^x$, so

  $$Ae^x + Ae^x = e^x$$

  $\because$ Obviously, $A = \frac 1 2$

  $\therefore y_{p_1}(x) = \frac 1 2 e^x$

  For the equation $y'' + y = x^3 e^{0x}$, let $y_{p_2}(x) = Ax^3 + Bx^2 + Cx + D$.

  Then $y_{p_2}'(x) = 3Ax^2 + 2Bx + C, y_{p_2}''(x) = 6Ax + 2B$, so

  $$Ax^3 + Bx^2 + (6A + C)x + 2B + D = x^3$$

  $\therefore A = 1, C = -6, B = D = 0$

  $\therefore y_{p_2}(x) = x^3 - 6x$

  $\therefore$ the general solution is

  $$\begin{aligned}
    y &= y_c + y_{p_1} + y_{p_2} \\
      &= C_1 \cos x + C_2 \sin x + \frac 1 2 e^x + x^3 - 6x
  \end{aligned}$$

  $\because y(0) = C_1 + \frac{1}{2} = 2, y'(0) = C_2 + \frac{1}{2} -6 = 0$

  $\therefore C_1 = \frac{3}{2}, C_2 = \frac{11}{2}$

  $\therefore$ the general solution is

  $$y = \frac{3}{2} \cos x + \frac{11}{2} \sin x + \frac{1}{2}e^x + 3x^2 - 6x$$

  \subsection*{8. }

  The auxiliary equation $\lambda ^2  - 4 \lambda = 0$, with roots $\lambda = 4$ and $\lambda = 0$

  For the equation $y'' - 4y = 0$, $y_c = C_1 + C_2 e^{4x}$

  For the equation $y'' - 4y = e^x \cos x$, let $y_p(x) = Ae^x \cos x + Be^x \sin x$

  Then $y_p'(x) = Ae^x(\cos x - \sin x) + Be^x (\sin x + \cos x)$

  Then $y_p ''(x) = Ae^x (\cos x - \sin x - \sin x - \cos x) + Be^x (\sin x + \cos x + \cos x - \sin x)$

  Then $y_p'' (x) = -2Ae^x \sin x + 2Be^x \cos x$, so

  $$(-2A - 4B)e^x \sin x + (2B - 4A)e^x \cos x  = e^x \cos x$$

  Since $-2A - 4B = 0, 2B - 4A = 1$, $A = -\frac{1}{5}, B = \frac{1}{10}$

  Therefore, $y_p(x) = -\frac{1}{5}e^x \cos x + \frac{1}{10}e^x \sin x$

  $\therefore$ the general solution is

  $$\begin{aligned}
    y &= y_c + y_p \\
      &= C_1 + C_2 e^{4x} -\frac{1}{5}e^x \cos x + \frac{1}{10}e^x \sin x
  \end{aligned}
  $$

  $\because y(0) = C_1 + C_2 - \frac{1}{5} = 2, y'(0) = 4C_2 - \frac{1}{5}(1-0) + \frac{1}{10}(0+1) = 4C_2 - \frac{1}{10} = 2$

  $\therefore C_2 = \frac{21}{40}, C_1 = \frac{67}{40}$

  $\therefore$ the general solution is

  $$y = \frac{67}{40} + \frac{21}{40}e^{4x} - \frac{1}{5}e^x \cos x + \frac{1}{10}e^x \sin x$$

  \subsection*{9. }

  The auxiliary equation is $\lambda^2 - \lambda = 0$, with roots $\lambda = 0$ and $\lambda = 1$

  For the equation $y'' - y' = 0$, $y_c = C_1 + C_2e^x$

  For the equation $y'' - y' = xe^x$, let $y_p(x) = (Ax^2 + Bx)e^x$

  Then $y_p'(x) = e^x (Ax^2 + Bx + 2Ax + B)$

  Then $y_p''(x) = e^x(Ax^2 + Bx + 2Ax + B + 2Ax + B + 2A)$, so

  $$e^x(2Ax + B + 2A) = xe^x$$

  Since $2A = 1, B + 2A = 0$, $A = \frac{1}{2}, B = -1$

  $\therefore$ the general solution is

  $$\begin{aligned}
    y &= y_c + y_p \\
      &= C_1 + C_2 e^x + (\frac{1}{2}x^2 - x)e^x
  \end{aligned}
  $$

  $\because y(0) = C_1 + C_2 = 2, y'(0) = C_2 + (-1) = 1$

  $\therefore C_2 = 2, C_1 = 0$

  $\therefore$ the general solution is

  $$y = 2e^x + (\frac{1}{2} x^2 - x)e^x$$

  \subsection*{16. }

  The auxiliary equation is $\lambda^2 + 3\lambda - 4 = 0$, with roots $\lambda = -4$ and $\lambda = 1$

  For equation $y'' + 3y' -4y = 0$, $y_c = C_1 e^x + C_2e^{-4x}$

  For equation $y'' + 3y' - 4y = x^3e^x$, let $y_{p_1}(x) = x(Ax^3 + Bx^2 + Cx + D)e^x$

  For equation $y'' + 3y' - 4y = xe^x$, let $y_{p_2}(x) = x(Ex + F)e^x$

  $\therefore$ the trial solution is

  $$\begin{aligned}
    y &= y_c + y_{p_1} + y_{p_2} \\
      &= C_1e^x + C_2e^{-4x} + (Ax^3 + Bx^2 + Cx + Ex + D + F)xe^x
  \end{aligned}
  $$

  \subsection*{17. }

  The auxiliary equation is $\lambda^2 + 2\lambda + 10 = 0$, with $\Delta = \sqrt{-36}$

  Therefore, the solution is $\lambda = \frac{-2 + 6i}{2} = -1 + 3i$ or $\lambda = \frac{-2 - 6i}{2} = -1 - 3i$

  For the equation $y'' + 2y' + 10y = 0$, $y_c = e^{-x}(C_1 \cos 3x + C_2 \sin 3x)$

  For the equation $y'' + 2y' + 10y = x^2 e^{-x} \cos 3x,$

  let $y_p = e^{-x} [(Ax^2 + Bx + C) \cos 3x + (Dx^2 + Ex + F) \sin 3x]$

  $\because \cos 3x, \sin 3x$ are solutions to $y_c$

  $\therefore$ the trial solution is

  $$\begin{aligned}
    y &= y_c + x y_p \\
      &= \{[C_1 + x(Ax^2 + Bx + C)] \cos 3x + [C_2 + x(Dx^2 + Ex + F)] \sin 3x] \}e^{-x}
  \end{aligned}
  $$

  \subsection*{18. }

  The auxiliary equation $\lambda^2 + 4 = 0$, with complex roots $\lambda = \pm 2i$

  For the equation $y'' + 4y = 0$, $y_c = C_1 \cos 2x + C_2 \sin 2x$
  
  For the equation $y'' + 4y = e^{3x}$, let $y_{p_1} = Ae^{3x}$

  For the equation $y'' + 4y = x \sin 2x$, let $y_{p_2} = (Bx + C) \sin 2x + (Dx + E) \cos 2x$

  $\because \sin 2x, \cos 2x$ are solutions to $y_c$ 

  $\therefore$ the trial solution is

  $$\begin{aligned}
    y &= y_c + y_{p_1} + xy_{p_2} \\
      &= Ae^{3x} + (Bx^2 + Cx + C_2) \sin 2x + (Dx^2 + Ex + C_1) \cos 2x
  \end{aligned}
  $$

  \subsection*{23. }

  The auxiliary equation is $\lambda^2 + 1 = 0$, with complex roots $\lambda = \pm i$

  For the equation $y'' + y = 0$, $y_c = C_1 \cos x + C_2 \sin x$

  Let $y_p(x) = u_1(x) \cos x + u_2(x) \sin x$

  $y_p'(x) = u_1'(x) \cos x + u_2'(x) \sin x - u_1(x) \sin x + u_2(x) \cos x$

  Impose the constraint that $u_1'(x) \cos x + u_2'(x) \sin x = 0$, then

  $y_p''(x) = -u_1'(x) \sin x + u_2'(x) \cos x - u_1(x) \cos x - u_2(x) \sin x$

  $$-u_1'(x) \sin x + u_2'(x) \cos x = \sec^2 x$$

  $$u_1'(x) = \frac{\biggl| \begin{matrix}
      0 & \sin x \\
      \sec^2 x & \cos x
  \end{matrix} \biggl|
  }{\biggl| \begin{matrix}
    \cos x & \sin x \\
    -\sin x & \cos x
\end{matrix} \biggl|} = -\sin x \sec^2 x = -\tan x \sec x$$

$$u_1(x) = -\sec x + C_3$$
  
  $$u_2'(x) = \frac{\biggl| \begin{matrix}
      \cos x & 0 \\
      -\sin x & \sec^2 x
  \end{matrix} \biggl|
  }{\biggl| \begin{matrix}
    \cos x & \sin x \\
    -\sin x & \cos x
\end{matrix} \biggl|} = \cos x \sec^2 x = \sec x = \frac{1}{\cos x}$$

$$u_2(x) = \ln (\sec x + \tan x) + C_4$$

$$\therefore y_p(x) = (-\sec x + C_3) \cos x + (\ln (\sec x + \tan x) + C_4) \sin x$$

$\therefore$ the solution is

$$y = (-\sec x + C_3 + C_1) \cos x + (\ln (\sec x + \tan x) + C_4 + C_2) \sin x$$
  
  \subsection*{25. }

  The auxiliary equation is $\lambda^2 - 3\lambda + 2 = 0$, with roots $\lambda = 1$ and $\lambda = 2$

  For the equation $y'' - 3y' + 2y = 0$, $y_c = C_1 e^x + C_2e^{2x}$

  Let $y_p(x) = u_1(x) e^{x} + u_2(x) e^{2x}$

  Then $y_p'(x) = u_1'(x) e^{x} + u_2'(x) e^{2x} + u_1(x) e^{x} + 2u_2(x) e^{2x}$

  Impose the constraint that $u_1'(x) e^{x} + u_2'(x) e^{2x} = 0$

  Then $y_p''(x) = u_1'(x) e^{x} + 2u_2'(x) e^{2x} + u_1(x) e^{x} + 4u_2(x) e^{2x}$

  $$u_1'(x) e^{x} + 2u_2'(x) e^{2x} + u_1(x) e^{x} + 4u_2(x) e^{2x} - 3u_1(x)e^x -6u_2(x)e^{2x} + 2u_1(x)e^x + 2u_2(x)e^{2x} = \frac{1}{1 + e^{-x}}$$

  $$u_1'(x) e^{x} + 2u_2'(x) e^{2x}  = \frac{1}{1 + e^{-x}}$$

  $$\because u_1'(x) e^x + u_2'(x)e^{2x} = 0$$

  $$u_1'(x) = \frac{-e^{-x}}{1 + e^{-x}}, u_2'(x) =\frac{e^{-2x}}{1 + e^{-x}}$$

  $$u_1(x) = \ln (1 + e^{-x}), u_2(x) = -e^{-x} + \ln (1 + e^{-x})$$

  $\therefore$ the general solution is

  $$y = C_1 e^x + C_2e^{2x} + \ln (1 + e^{-x)e^x + (-e^{-x} + \ln(1 + e^{-x}))e^{2x}$$

\end{document}
