
\documentclass{article}
\usepackage{amsmath}
\usepackage{amsthm}
\usepackage{amssymb}
\usepackage{enumerate}
\usepackage{tikz}
\usepackage{graphicx}

\begin{document}
  \title{Exercise 15.8 \& 15.9}
  \author{Wang Yue from CS Elite Class}
  \maketitle

  \section*{15.8}

  \subsection*{18. }

  $D = \{ (x, y, z) | x^2 + y^2 \leq z, 0 \leq z \leq 4 \}$

  $$\begin{aligned}
    \iiint_E z dV &= \int_0^{2\pi} \int_0^4 \int_0^{\sqrt z} zr dr dz d\theta \\
    &= \int_0^{2\pi} \int_0^4 z (\frac{r^2}{2})\biggl|_0^{\sqrt z} dz d\theta \\
    &= \frac 1 2 \int_0^{2\pi} \int_0^4 z^2 dz d\theta \\
    &= \frac 1 2 \int_0^{2\pi} \frac{z^3}{3}\biggl|_0^4 d\theta \\
    &= \frac 1 6 \int_0^{2\pi} \frac{64}{3} d\theta \\
    &= \frac{64\pi}{9}
  \end{aligned}$$

  \subsection*{19. }

  $D = \{ (x, y, z) | 0 < x > 2, 0 < y < 2, 0 < z < 4 - x^2 - y^2 \}$

  $$\begin{aligned}
    \iiint_E (x + y + z) dV &= \int_0^{2\pi} \int_0^4 \int_0^{\sqrt{4-z}} (r\cos \theta + r\sin \theta + z) r dr dz d\theta \\
    &= \int_0^{2\pi} \int_0^4 (\cos \theta + \sin \theta)(\frac{r^3}{3})\biggl|_0^{\sqrt{4-z}} + z(\frac{r^2}{2})\biggl|_0^{\sqrt{4-z}} dz d\theta \\
    &= -\int_0^{2\pi} \int_0^4 \frac{(4-z)^{\frac 3 2}}{3}(\cos \theta + \sin \theta) + \frac{z(4-z)}{2} d(4-z) d\theta \\
    &= -\int_0^{2\pi} \frac{\cos \theta + \sin \theta}{3} \frac 2 5 (4-z)^{\frac 5 2}\biggl|_0^{4} d\theta + \int_0^{2\pi} \int_0^4 (2z - \frac{z^2}{2}) dz d\theta \\
    &= \int_0^{2\pi} \frac{\cos \theta + \sin \theta}{3} \frac{64}{5} d\theta + \int_0^{2\pi} (z^2 - \frac{z^3}{6})\biggl|_0^4 d\theta \\
    &= \frac{64}{15} (\sin \theta - \cos \theta)\biggl|_0^{2\pi} + \int_0^{2\pi} (16 - \frac{32}{3})d\theta \\
    &= \frac{32\pi}{3}
  \end{aligned}$$

  \subsection*{20. }

  $$\begin{aligned}
    \iiint_E x dV &= \int_0^{2\pi} \int_2^3 \int_0^{r\cos \theta + r\sin \theta + 5} xr dz dr d\theta \\
    &= \int_0^{2\pi} \int_2^3 r^2 \cos \theta (r\cos \theta + r\sin \theta + 5) dr d\theta \\
    &= \int_0^{2\pi} \int_2^3 (r^3\cos^2 \theta + r^3 \sin \theta \cos \theta + 5r^2\cos \theta) dr d\theta  \\
    &= \int_0^{2\pi} (\frac{r^4(\cos^2 \theta + \sin \theta \cos \theta)}{4} + \frac{5r^3\cos \theta}{3})\biggl|_2^3 d\theta \\
    &= \int_0^{2\pi} \frac{65 \cos^2 \theta + 65\sin \theta \cos \theta}{4} + \frac{95\cos \theta}{3} d\theta \\
    &= \int_0^{2\pi} \frac{65+65\cos 2\theta}{8} d\theta + \int_0^{2\pi}\frac{65\sin \theta}{4} d\sin \theta \\
    &= \frac{65\pi}{4} + \frac{65}{4} (\frac{\sin^2 \theta}{2})\biggl|_0^{2\pi} = \frac{65\pi}{4}
  \end{aligned}$$

  \subsection*{21. }

  $$\begin{aligned}
    \iiint_E x^2 dV &= \int_0^{2\pi} \int_0^1 \int_0^{2r} (r^3 \cos^2 \theta ) dz dr d\theta \\
    &= \int_0^{2\pi} \int_0^1 (2r^4\cos^2 \theta) dr d\theta \\
    &= 2\int_0^{2\pi} \cos^2 \theta (\frac{r^5}{5})\biggl|_0^1 d\theta \\
    &= \frac 2 5 \int_0^{2\pi} \cos^2 \theta d\theta \\
    &= \frac 1 5 \int_0^{2\pi} \frac 1 2 (1 + \cos 2\theta) d(2\theta) \\
    &= \frac 1 5 \frac 1 2 (2 \theta + \sin 2\theta)\biggl|_0^{2\pi} \\
    &= \frac{2\pi}{5}
  \end{aligned}$$

  \subsection*{24. }

  Let $z = 2 - z^2$, then $z = -2$ (abandoned) or $z = 1$

  $$\begin{aligned}
    V &= \int_0^{2\pi} \int_0^1 \int_0^z r dr dz d\theta \\
    &= \int_0^{2\pi} \int_0^1 (\frac{r^2}{2})\biggl|_0^z dz d\theta \\
    &= \frac 1 2 \int_0^{2\pi} \int_0^1 z^2 dz d\theta \\
    &= \frac 1 2 \int_0^{2\pi} \frac{z^3}{3}\biggl|_0^1 d\theta \\
    &= \frac{\pi}{3} 
  \end{aligned}$$

  \subsection*{29. }

  $$\begin{aligned}
    \int_{-2}^2 \int_{-\sqrt{4-y^2}}^{\sqrt{4-y^2}} \int_{\sqrt{x^2+y^2}}^2 xz dz dx dy &= \int_0^{2\pi} \int_0^2 \int_r^2 (zr^2 \cos \theta) dz dr d\theta \\
    &= \int_0^{2\pi} \int_0^2 r^2\cos \theta (\frac{z^2}{2})\biggl|_r^2 dr d\theta \\
    &= \int_0^{2\pi} \int_0^2 (2r^2 - \frac{r^4}{2})\cos \theta  dr d\theta \\
    &= \int_0^{2\pi} \int_0^2 \cos \theta (\frac{2r^3}{3} - \frac{r^5}{10})\biggl|_0^2 d\theta \\
    &= \frac{32}{15}\int_0^{2\pi} \cos \theta  d\theta \\
    &= 0
  \end{aligned}$$

  \section*{15.9}

  \subsection*{25. }

  $$\begin{aligned}
    \iiint_E xe^{x^2+y^2+z^2} dV &= \int_0^{\frac \pi 2} \int_0^{\frac \pi 2} \int_0^1 (\rho \sin \varphi \cos \theta e^{\rho^2} \rho^2 \sin \varphi) d\rho d\theta d\varphi \\
    &= \int_0^{\frac \pi 2} \int_0^{\frac \pi 2} \int_0^1 (e^{\rho^2} \rho^3 \sin^2 \varphi \cos \theta) d\rho d\theta d\varphi \\
    &= \int_0^{\frac \pi 2} \int_0^{\frac \pi 2} \sin^2 \varphi \cos \theta \int_0^1 (\frac 1 2 e^{\rho^2} \rho^2) d\rho^2 d\theta d\varphi \\
    &= \frac 1 2 \int_0^{\frac \pi 2} \int_0^{\frac \pi 2} \sin^2 \varphi \cos \theta (\rho^2 e^{\rho^2})\biggl|_{\rho=0}^{\rho=1} d\theta d\varphi \\
    &= \frac e 2 \int_0^{\frac \pi 2} \int_0^{\frac \pi 2} \sin^2 \varphi \cos \theta d\theta d\varphi \\
    &= \frac e 2 \int_0^{\frac \pi 2} \sin^2 \varphi (\sin \theta)\biggl|_0^{\frac \pi 2} d\varphi \\
    &= \frac e 2 \int_0^{\frac \pi 2} \frac{1 - \cos 2\varphi}{2} d\varphi \\
    &= \frac e 2 (\frac \varphi 2 + \frac{2\sin 2\varphi }{2})\biggl|_0^{\frac \pi 2} \\
    &= \frac{e\pi}{8} 
  \end{aligned}$$

  \subsection*{27. }

  $$\begin{aligned}
    \int_{\frac \pi 6}^{\frac \pi 3} \int_0^{2\pi} \int_0^a \rho^2 \sin \varphi d\rho d\theta d\varphi &= \int_{\frac \pi 6}^{\frac \pi 3} \int_0^{2\pi} \sin \varphi (\frac{\rho^3}{3})\biggl|_0^a d\theta d\varphi \\
    &= \frac{2\pi a^2}{3} \int_{\frac \pi 6}^{\frac \pi 3} \sin \varphi d\varphi \\
    &= \frac{2\pi a^2}{3} (-\cos \varphi)\biggl|_{\frac \pi 6}^{\frac \pi 3} \\
    &= \frac{2\pi a^2}{3} \times \frac{\sqrt 3 - 1}{2} \\
    &= \frac{(\sqrt 3 - 1)\pi a^2}{3}
  \end{aligned}$$

  \subsection*{30. }

  Let $x^2 + y^2 + (\sqrt{x^2 + y^2})^2 = 4$, then $x^2 + y^2 = z^2 = 2$, $z = \sqrt 2$

  $$\begin{aligned}
    \therefore V &= \int_{\frac \pi 4}^{\frac \pi 2} \int_0^{2\pi} \int_0^2 (\rho^2 \sin \varphi) d\rho d\theta d\varphi \\
    &= \int_{\frac \pi 4}^{\frac \pi 2} \int_0^{2\pi} \sin \varphi (\frac{\rho^3}{3})\biggl|_0^2 d\theta d\varphi \\
    &= \frac 8 3 \int_{\frac \pi 4}^{\frac \pi 2} \int_0^{2\pi} \sin \varphi d\theta d\varphi \\
    &= \frac{16\pi}{3} \int_{\frac \pi 4}^{\frac \pi 2} \sin \varphi d\varphi \\
    &= \frac{16\pi}{3} (\cos \varphi)\biggl|_{\frac \pi 2}^{\frac \pi 4} \\
    &= \frac{8\sqrt 2\pi}{3} \\
  \end{aligned}$$
  
  \subsection*{39. }

  $$\begin{aligned}
    \int_0^1 \int_0^{\sqrt{1-x^2}}\int_{\sqrt{x^2 + y^2}}^{\sqrt{2-x^2 - y^2}} xy dz dy dx &= \int_0^{\frac \pi 3} \int_0^{\frac \pi 2} \int_0^2 (\rho^4 \sin^3 \varphi \sin \theta \cos \theta) d\rho d\theta d\varphi \\
    &= \int_0^{\frac \pi 3} \int_0^{\frac \pi 2} \sin^3 \varphi \sin \theta \cos \theta (\frac{\rho^5}{5})\biggl|_0^2 d\theta d\varphi \\
    &= \frac{16}{5} \int_0^{\frac \pi 3} \int_0^{\frac \pi 2} \sin^3 \varphi \sin \theta \cos \theta d\theta d\varphi \\
    &= \frac{16}{5} \int_0^{\frac \pi 3} \int_0^{\frac \pi 2} \sin^3 \varphi \sin \theta d\sin \theta d\varphi \\
    &= \frac{16}{5} \int_0^{\frac \pi 3} \sin^3 \varphi (\frac{\sin^2 \theta}{2})\biggl|_0^{\frac \pi 2} d\varphi \\
    &= \frac{8}{5} \int_0^{\frac \pi 3} (\cos^2 \varphi - 1) d\cos \varphi \\
    &= \frac{8}{5} (\frac{\cos^3 \varphi}{3} - \cos \varphi)\biggl|_0^{\frac \pi 3} \\
    &= \frac 8 5 (\frac{1}{24} - \frac 1 2 - \frac 1 3 + 1) \\
    &= \frac 8 5 \times \frac{5}{24} = \frac 1 3 \\
  \end{aligned}$$

  \subsection*{41. }

  The center of the sphere is $(0, 0, 2)$, then we have

  $$x^2 + y^2 + (z-2)^2 = 4$$

  Change into spherical coordinate, then $$\rho^2 \sin^2 \varphi + \rho^2 \cos^2 \varphi = \rho^2 = 4\rho \cos \varphi \implies \rho = 4\cos \varphi$$

  $$\begin{aligned}
    \int_{-2}^2 \int_{-\sqrt{4-x^2}}^{\sqrt{4-x^2}} \int_{2-\sqrt{4-x^2-y^2}}^{2 + \sqrt{4-x^2-y^2}} (x^2 + y^2 + z^2)^{\frac 3 2} dz dy dx &= \int_0^{\pi} \int_0^{2\pi} \int_0^{4\cos \varphi} (\rho^3 \rho^2 \sin \varphi) d\rho d\theta d\varphi \\
    &= \int_0^{\pi} \int_0^{2\pi} \sin \varphi (\frac{\rho^6}{6})\biggl|_0^{4\cos \varphi} d\theta d\varphi \\
    &= \int_0^{\pi} \int_0^{2\pi} \sin \varphi \frac{(4\cos \varphi)^6}{6} d\theta d\varphi \\
    &= \frac{4^6 \pi}{3} \int_0^{\pi} \sin \varphi (\cos \varphi)^6  d\varphi \\
    &= -\frac{4^6 \pi}{3} \int_0^{\pi} \cos^6 \varphi d\cos \varphi \\
    &=  -\frac{4^6 \pi}{3} (\frac{\cos^7 \varphi}{7})\biggl|_0^{\pi} \\
    &= \frac{2^{13}\pi}{21}
  \end{aligned}$$

\end{document}