\documentclass{article}
\usepackage{amsmath}
\usepackage{amsthm}
\usepackage{amssymb}
\usepackage{enumerate}
\usepackage{tikz}
\usepackage{graphicx}

\begin{document}
  \title{Exercise 9.3}
  \author{Wang Yue from CS Elite Class}
  \maketitle

  \subsection*{12. $\frac{dy}{dx} = \frac{\ln x}{xy}, y(1) = 2$}

  $$\frac{\ln x}{x} dx = \ln x d \ln x = y dy$$

  $$\int \ln x d\ln x = \int y dy$$

  $$\frac{(\ln x)^2}{2} = \frac{y^2}{2} + C$$

  $\because \frac{(\ln 1)^2}{2} = 2 + C$

  $\therefore C = -2$

  $$\therefore y^2 = (\ln x)^2 + 4$$

  \subsection*{14. $ y' = \frac{xy \sin x}{y + 1}, y(0) = 1 $}

  $$\frac{dy}{dx} = \frac{xy \sin x}{y + 1}$$

  If $y \not = 0$, then

  $$\frac{y+1}{y}dy = x \sin x dx$$

  $$\int \frac{y+1}{y}dy = \int x \sin x dx$$

  $$y + \ln |y| = -\int x d\cos x = -x\cos x + \sin x + C$$

  $\because 1 + \ln 1 = -0 + 0 + C$

  $\therefore C = 1$

  $$\therefore y + \ln |y| = -x\cos x + \sin x + 1$$

  $\because y = 0$ satisfies $\frac{dy}{dx} = \frac{xy \sin x}{y + 1} = 0$

  $\therefore \left\{ \begin{array}{ll} y + \ln |y| = -x\cos x + \sin x + 1, & y \not = 0 \\ y = 0, &y = 0 \end{array}\right.$

  \subsection*{20. $ f'(x) = f(x)(1-f(x)), f(0) = \frac 1 2 $}

  $$\frac{dy}{dx} = y(1-y)$$

  If $y \not = 0$ and $y \not = 1$, then

  $$\int \frac{1}{y(1-y)} dy = \int dx$$

  $$\int (\frac{1}{y} + \frac{1}{1 - y}) dy = \ln |y| + \ln |1-y| = x + C$$

  $$e^{\ln |y|} e^{\ln |1-y|} = |y||1-y| = e^C e^x$

  $\because \frac 1 4 = e^C$

  $\therefore |y| |1-y| = \frac 1 4 e^x$

  If $y = 0$ or $y = 1$, then $\frac{dy}{dx} = 0$ is satisified

  $\therefore \left\{ \begin{array}{ll}
      |y| |1-y| = \frac 1 4 e^x, &y \not = 0 \textrm{ and } y \not = 1 \\
      y = 0, &y = 0 \\
      y = 1, &y = 1
  \end{array}\right.$

  \subsection*{22. $xy' = y + xe^{\frac y x}$}

  Let $v = \frac y x$, then $y = vx$, then

  $$y' = \frac{dy}{dx} = \frac{dv}{dx}x + v$$

  $$\therefore x \frac{dv}{dx} = e^v$$

  $$\int \frac{1}{e^v} dv = \int \frac 1 x dx$$

  $$-e^{-v} = \ln |x| + C$$

  where $C$ is an arbitrary constant

  \subsection*{33. $ y(x) = 2 + \int_2^x [t - ty(t)]dt $}

  Taking derivative on the both sides, we get

  $$\frac{dy}{dx} = x - xy$$

  and the initial condition is $y(2) = 2 + \int_2^2 [t-ty(t)] dt = 2$

  If $y \not = 1$, then

  $$\int \frac{1}{1-y} dy = \int x dx$$

  $$-\ln|1-y| = \frac{x^2}{2} + C$$

  $\because -\ln |1 - 2| = \frac{2^2}{2} + C$

  $\therefore C = -2$

  $$\therefore |\frac{1}{1-y}| = e^{-2} e^{\frac{x^2}{2}}$$

  If $y = 1$, then $\frac{dy}{dx} = 0$

  $\therefore \left\{ \begin{array}{ll} |\frac{1}{1-y}| = e^{-2} e^{\frac{x^2}{2}}, &y \not = 1 \\ y = 1, &y = 1 \end{array}\right.$

  \subsection*{34. }

  Taking derivative on the both sides, we get
  
  $$\frac{dy}{dx} = \frac{1}{xy}$$

  and the initial condition $y(1) = 2$

  $$\therefore \int y dy = \int \frac{1}{x} dx$$

  Since $x > 0$, then

  $$ \frac{y^2}{2} = \ln x + C_1 $$

  $$\therefore y^2 = 2\ln x + C$$

  where $C_1$ and $C$ is arbitrary constants

  \subsection*{35. }

  Taking derivative on the both sides, we get

  $$\frac{dy}{dx} = 2x \sqrt{y}$$

  and the initial condition $y(0) = 4$

  If $y > 0$, then

  $$\int \frac{1}{2\sqrt y} dy = \int x dx$$

  $$\sqrt y = \frac{x^2}{2} + C_1$$

  $$y = \frac{x^4}{4} + C$$

  $\because 4 = 0 + C$

  $\therefore C = 4$

  $$\therefore y = \frac{x^4}{4} + 4$$

  If $y = 0$, then $\frac{dy}{dx} = 0$

  $\therefore \begin{array}{ll}
    y = \frac{x^4}{4} + 4, &y \not = 0 \\
    y = 0, &y = 0
  \end{array}\right.$

\end{document}

