\documentclass{article}
\usepackage{amsmath}
\usepackage{amsthm}
\usepackage{amssymb}
\usepackage{enumerate}
\usepackage{graphicx}

\begin{document}
    \title{Exercise 14.4}
    \author{Wang Yue from CS Elite Class}
    \date{\today}
    \maketitle

    \subsection*{21. Find the linear approximation of $f(x, y, z) = \sqrt{x^2+y^2+z^2}$ at $(3, 2, 6)$. Approximate $\sqrt{(3.02)^2+(1.97)^2+(5.99)^2}$.}

    $$f_x(x, y, z) = \frac{x}{\sqrt{x^2+y^2+z^2}}$$

    $$f_y(x, y, z) = \frac{y}{\sqrt{x^2+y^2+z^2}}$$

    $$f_z(x, y, z) = \frac{z}{\sqrt{x^2+y^2+z^2}}$$

    Therefore, the linear approximation of $f$ is

    $$\begin{aligned}
        &f(3, 2, 6) + f_x(3, 2, 6)(x-3) + f_y(3, 2, 6)(y - 2) + f_z(3, 2, 6)(z-6) \\ 
        &= 7 + \frac{3(x-3) + 2(y-2) + 6(z-6)}{7} \\
    \end{aligned}$$

    When $x = 3.02, y=1.97, z=5.99$, $f(x, y, z) \approx 7 + \frac{0.06 - 0.06 - 0.06}{7} \approx 6.99$

    \subsection*{25. $z = e^{-2x} \cos 2\pi t$}

    $$\frac{\partial z}{\partial x} = -2 e^{-2x}\cos 2\pi t, \quad \frac{\partial z}{\partial t} = -2\pi e^{-2x}\sin 2\pi t$$

    $$dz = \frac{\partial z}{\partial x}dx + \frac{\partial z}{\partial r}dr = -2e^{-2x}\cos 2\pi t dx - 2\pi e^{-2x} \sin 2\pi t dt$$

    \subsection*{28. $T = \frac{v}{1+uvw}$}

    $$\frac{\partial T}{\partial u} = \frac{-v^2w}{(1+uvw)^2}, \quad \frac{\partial T}{\partial w} = \frac{-v^2u}{(1+uvw)^2}$$

    $$\frac{\partial T}{\partial v} = \frac{1(1+uvw) - v(uw)}{(1+uvw)^2} = \frac{1}{(1+uvw)^2}$$

    $$dT = \frac{\partial T}{\partial u} du + \frac{\partial T}{\partial v} dv + \frac{\partial T}{\partial w} dw = \frac{-v^2w du  + dv- v^2u dw}{(1+uvw)^2}$$

    \subsection*{30. $L = xze^{-y^2-z^2}$}

    $$\frac{\partial L}{\partial x} = ze^{-y^2-z^2}, \quad \frac{\partial L}{\partial y} = -2xyze^{-y^2-z^2}, \quad \frac{\partial L}{\partial z} = x(1 -2z^2)e^{-y^2-z^2}$$

    $$dL = \frac{\partial L}{\partial x} dx + \frac{\partial L}{\partial y} dy + \frac{\partial L}{\partial z} dz = \frac{zdx - 2xyzdy + x(1-2z^2)dz}{e^{y^2+z^2}}$$

    \subsection*{42.}
    
    First, find the tangent lines of $\overrightarrow{r_1}$ and $\overrightarrow{r_2}$.

    $$\frac{d\overrightarrow{r_1}}{dt} = \langle 3, -2t, 2t - 4 \rangle$$

    $\because \overrightarrow{r_1}(0) = (2, 1, 3), \quad \therefore \overrightarrow{r_1'}(0) = (3, 0, -4)$

    $$\frac{d\overrightarrow{r_2}}{dt} = \langle 2u, 6u^2, 2 \rangle$$

    $\because \overrightarrow{r_2}(1) = (2, 1, 3), \quad \therefore \overrightarrow{r_2'}(1) = (2, 6, 2)$

    $$\therefore \overrightarrow{n} = \overrightarrow{r_1}(0) \times \overrightarrow{r_2}(1) = (-16, 2, 10)$$

    $\therefore$ the equation of the tangent plane at $P$ is $-16(x-2) + 2(y-1) + 10(z-3) = 0$, or

    $$8x-y + 5z= 30$$
    
    \subsection*{45.}

    $\because$ by the definition of linear approximation, 

    $$f(a + \Delta x, b + \Delta y) = f(a, b) + f_x(a, b)\Delta x + f_y(a, b)\Delta y + o(\sqrt{(\Delta x)^2 + (\Delta y)^2})$$

    $$\therefore \lim_{(\Delta x, \Delta y) \to (0, 0)} f(a + \Delta x, b + \Delta y) = f(a, b)$$

    $\because f$ is differentiable,

    $\therefore f$ is continuous at $(a, b)$.

    \subsection*{46.}

    \begin{enumerate}[(a)]
        \item 

        $$f_x(0, 0) = \lim_{h \to 0}\frac{f(h, 0) - f(0, 0)}{h} = \lim_{h \to 0}\frac{0 - 0}{h} = 0$$

        $$f_y(0, 0) = \lim_{h \to 0}\frac{f(0, h) - f(0, 0)}{h} = \lim_{h \to 0}\frac{0 - 0}{h} = 0$$

        $$\lim_{(\Delta x, \Delta y) \to (0, 0)}f(0 + \Delta x, 0 + \Delta y) = \lim_{(\Delta x, \Delta y) \to (0, 0)}\frac{\Delta x \Delta y}{(\Delta x)^2 + (\Delta y)^2}$$

        Let $\Delta y = k\Delta x$, then $$\lim_{(\Delta x, \Delta y) \to (0, 0)}\frac{k(\Delta x)^2}{(1+k^2)(\Delta x)^2} = \frac{k}{1 + k^2} \not = 0\textrm{ when } k \not = 0$$

        $\therefore \lim_{(\Delta x, \Delta y) \to (0, 0)}f(\Delta x, \Delta y)$ does not exist.

        $\therefore f$ is not continuous at $(0, 0)$.

        $\therefore$ by the result of T45, $f$ is not differentiable.

        \item 

        $\because f$ is not differentiable at $(0, 0)$

        $\therefore f_x$ and $f_y$ are not continuous at $(0, 0)$
    \end{enumerate}

\end{document}