\documentclass{article}
\usepackage{amsmath}
\usepackage{amsthm}
\usepackage{amssymb}
\usepackage{enumerate}
\usepackage{graphicx}

\begin{document}
    \title{Exercise 11.10}
    \author{Wang Yue from CS Elite Class}
    \date{March 28, 2021}
    \maketitle

    \subsection*{47. $\int x \cos(x^3) \textrm dx$}

    $\because \cos x = 1 - \frac{x^2}{2} + \frac{x^4}{4!} - \cdots = \sum_{n=0}^\infty (-1)^n \frac{x^{2n}}{(2n)!}$

    $\therefore x \cos(x^3) = \sum_{n=0}^\infty (-1)^n \frac{x^{6n+1}}{(2n)!}$

    $\therefore \int x \cos (x^3) \textrm dx = \sum_{n=0}^\infty (-1)^n \int \frac{x^{6n+1}}{(2n)!} \textrm dx$

    $= \sum_{n=0}^\infty (-1)^n \frac{x^{6n+2}}{(6n+2)(2n)!} + C$

    where C is a constant.

    \subsection*{50. $\int \arctan(x^2) \textrm dx$}

    $\because \arctan x = x - \frac{x^3}{3} + \frac{x^5}{5} - \frac{x^7}{7} + \cdots = \sum_{n=0}^\infty (-1)^n \frac{x^{2n+1}}{(2n+1)!}$

    $\therefore \int \arctan(x^2) \textrm dx = \int \sum_{n=0}^\infty \frac{x^{4n+2}}{(2n+1)!} \textrm dx$

    $ = \sum_{n=0}^\infty \int \frac{x^{4n+2}}{(2n+1)!} \textrm dx$

    $ = \sum_{n=0}^\infty \frac{x^{4n+3}}{(4n+3)(2n+1)!} + C$

    \subsection*{55. $\lim_{x\to 0}\frac{x - \ln(1+x)}{x^2}$}

    $\ln(1+x) = x - \frac{x^2}{2} + \frac{x^3}{3} - \frac{x^4}{4} + \cdots = \sum_{n=1}^\infty (-1)^n \frac{x^n}{n}$

    $$\begin{aligned}
        \lim_{x\to 0}\frac{x - \ln(1+x)}{x^2} &= \lim_{x\to 0}\frac{x - (x - \frac{x^2}{2} + \frac{x^3}{3} - \frac{x^4}{4} + \cdots)}{x^2} \\
        &= \lim_{x\to 0}\frac{\frac{x^2}{2} - \frac{x^3}{3} + \frac{x^4}{4} - \cdots}{x^2} \\
        &= \lim_{x\to 0}(\frac{1}{2} - \frac{x}{3} + \frac{x^2}{4} - \frac{x^3}{5} + \cdots) \\
        &= \frac 1 2
    \end{aligned}$$

    \subsection*{56. $\lim_{x\to 0}\frac{1 - \cos x}{1 + x - e^x}$}

    $\cos x = 1 - \frac{x^2}{2} + \frac{x^4}{4!} - \cdots = \sum_{n=0}^\infty (-1)^n \frac{x^{2n}}{(2n)!}$

    $e^x = 1 + x + \frac{x^2}{2} + \cdots = \sum_{n=0}^\infty \frac{x^n}{n!}$

    $$\begin{aligned}
        \lim_{x\to 0}\frac{1 - \cos x}{1 + x - e^x} &= \lim_{x\to 0}\frac{-\sum_{n=1}^\infty (-1)^n \frac{x^{2n}}{(2n)!}}{-\sum_{n=2}^\infty \frac{x^n}{n!}} \\
        &= \frac{\frac{x^2}{2!} - \frac{x^4}{4!} + \frac{x^6}{6!} - \frac{x^8}{8!} + \cdots}{\frac{x^2}{2!} + \frac{x^3}{3!} + \frac{x^4}{4!} + \cdots} \\
        &= 1
    \end{aligned}$$

    \subsection*{57. $\lim_{x\to 0}\frac{\sin x - x + \frac 1 6 x^3}{x^5}$}

    $\sin x = x - \frac{x^3}{3!} + \cdots = \sum_{n=0}^\infty (-1)^n \frac{x^{2n+1}}{(2n+1)!}$

    $$\begin{aligned}
        \lim_{x\to 0}\frac{\sin x - x + \frac 1 6 x^3}{x^5} &= \lim_{x\to 0}\frac{\frac{x^5}{5!} - \frac{x^7}{7!} + \cdots}{x^5} \\
        &= \lim_{x\to 0}(\frac{1}{5!} - \frac{x^2}{7!} + \frac{x^4}{9!} - \frac{x^6}{11!} + \cdots) \\
        &= \frac{1}{120} 
    \end{aligned}$$

    \subsection*{65. $\sum_{n=1}^\infty (-1)^{n-1} \frac{3^n}{n 5^n}$}

    More generally, let $f(x) = \sum_{n=1}^\infty (-1)^{n-1} \frac{x^n}{n} = x - \frac{x^2}{2} + \frac{x^3}{3} - \frac{x^4}{4} + \cdots = \ln (1 + x)$

    $\therefore \sum_{n=1}^\infty (-1)^{n-1} \frac{3^n}{n 5^n} = f(\frac 3 5) = \ln \frac 8 5$

    \subsection*{68. $1 - \ln 2 + \frac{(\ln 2)^2}{2!} - \frac{(\ln 2)^3}{3!} + \cdots$}      

    More generally, let $f(x) = 1 - x + \frac{x^2}{2!} - \frac{x^3}{3!} + \cdots = \sum_{n=0}^\infty \frac{(-x)^n}{n!} = e^{-x}$

    $\therefore 1 - \ln 2 + \frac{(\ln 2)^2}{2!} - \frac{(\ln 2)^3}{3!} + \cdots = f(\ln 2) = e^{-\ln 2} = \frac 1 2$

    \subsection*{70. $\frac{1}{1 \cdot 2} - \frac{1}{3 \cdot 2^3} + \frac{1}{5 \cdot 2^5} - \frac{1}{7 \cdot 2^7} + \cdots$}

    More generally, let $f(x) = \frac{x}{1} - \frac{x^3}{3} + \frac{x^5}{5} - \frac{x^7}{7} + \cdots = \arctan x$

    $\therefore \frac{1}{1 \cdot 2} - \frac{1}{3 \cdot 2^3} + \frac{1}{5 \cdot 2^5} - \frac{1}{7 \cdot 2^7} + \cdots = \arctan \frac 1 2$

    \subsection*{72. If $f(x) = (1+x^3)^{30}$, what is $f^{(58)}(0)$?}

    $\because (1+x)^k = \sum_{n=0}^{\infty} {k \choose n} x^n$

    $\therefore f(x) = (1 + x^3)^{30} = \sum_{n=0}^\infty {30 \choose n}x^{3n} = {30 \choose 0}x^0 + {30 \choose 1}x^3 + {30 \choose 2}x^6 + \cdots$

    $\therefore f^{(58)}(x) = {30 \choose 20}60 \times 59 \times \cdots \times 3 x^2 + {30 \choose 21}63 \times 62 \times \cdots \times 6 x^5 + \cdots$

    $\therefore f^{(58)}(0) = 0$

\end{document}