\documentclass{article}
\usepackage{amsmath}
\usepackage{amsthm}
\usepackage{amssymb}
\usepackage{enumerate}
\usepackage{graphicx}

\begin{document}
  \title{Exercise 14.7}
  \author{Wang Yue from CS Elite Class}
  \date{\today}
  \maketitle

  \subsection*{9. $f(x, y) = y^3 + 3x^2y - 6x^2 -6y^2 + 2$}

  $$f_x(x, y) = 6xy - 12x, f_y(x, y) = 3y^2+3x^2-12y$$

  Let $f_x(x, y) = f_y(x, y) = 0$, then $\left\{ \begin{array}{ll} x = 0 \\ y = 0 \end{array}\right.$ or $\left\{ \begin{array}{ll} x = \pm 2 \\ y = 2 \end{array}\right.$

  $$f_{xx} = 6y - 12, f_{yy} = 6y - 12, f_{xy} = 6x$$

  $$D = f_{xx}(x, y)f_{yy}(x, y) - [f_{xy}(x, y)]^2 = (6y-12)^2 - (6x)^2 = 36(y-2+x)(y-2-x)$$

  When $x = 0, y = 0$, $D = 36 \times (-2)^2 > 0, f_{xx}(0, 0) = -12 < 0$
  
  thus $f(0, 0)$ is a local maximum

  When $x = \pm 2, y = 2$, $D = 36 \times 2 \times (-2) < 0$

  thus $f(\pm 2, 2)$ is a saddle point, i.e. not a local maximum or local minimum

  \subsection*{15. $f(x, y) = (x^2+y^2)e^{y^2-x^2}$}

  $$f_x(x, y) = 2xe^{y^2-x^2} + (x^2+y^2)e^{y^2-x^2}(-2x) = 2xe^{y^2-x^2}(1-x^2-y^2)$$

  $$f_y(x, y) = 2ye^{y^2-x^2} + (x^2+y^2)e^{y^2-x^2}2y = 2ye^{y^2-x^2}(1+x^2+y^2)$$

  Let $f_x(x, y) = f_y(x, y) = 0$ , then $\left\{ \begin{array}{ll} x = 0 \\ y = 0 \end{array}\right.$ or $\left\{ \begin{array}{ll} x = \pm 1 \\ y = 0 \end{array}\right.$

  $$\begin{aligned}
    f_{xx}(x, y) &= 2e^{y^2-x^2}(1-x^2-y^2) + 2e^{y^2-x^2}(-2x)(1-x^2-y^2) + 2xe^{y^2-x^2}(-2x) \\ 
    &= 2e^{y^2-x^2}[(1-2x^2)(1-x^2-y^2) - 2x^2]
  \end{aligned}$$

  $$\begin{aligned}
    f_{yy}(x, y) &= 2e^{y^2-x^2}(1+x^2+y^2) + 2ye^{y^2-x^2}(2y)(1+x^2+y^2) + 2ye^{y^2-x^2}(2y) \\ 
    &= 2e^{y^2-x^2}[(1+2y^2)(1+x^2+y^2) + 2y^2]
  \end{aligned}$$

  $$\begin{aligned}
    f_{xy}(x, y) &= 2xe^{y^2-x^2}(2y)(1-x^2-y^2) + 2xe^{y^2-x^2}(-2y) \\ 
    &= 4xye^{y^2-x^2}(-x^2-y^2)
  \end{aligned}$$

  When $x = 0, y = 0$, $$D = f_{xx}(x, y)f_{yy}(x, y) - [f_{xy}(x, y)]^2 = 2 \times 2 - 0 = 4 > 0, \quad f_{xx}(x, y) > 0$$

  $\therefore f$ reach its minimum at $(0, 0)$

  When $x = \pm 1, y = 0$, $$D = (-4e^{-1}) \times 4e^{-1} - 0 < 0, \quad f_{xx}(x, y) < 0$$

  $\therefore (\pm 1, 0)$ are saddle points

  \subsection*{33. $f(x, y) = x^4+y^4-4xy+2, \quad D = \{ (x, y) | 0 \leq x \leq 3, 0 \leq y \leq 2 \}$}

  $$f_x(x, y) = 4x^3-4y, f_y(x, y) = 4y^3 - 4x$$

  Let $f_x(x, y) = f_y(x, y) = 0$, then $x = 1, y = 1$

  $f(0, y) = 0 + y^4 - 0 + 2 = x^4 + 2 \in [2, 83]$

  $f(x, 0) = y^4+2 \in [2, 18]$

  $f(3, y) = 81 + y^4 - 12y + 2 = y(y^3-12) + 83 \ in [3^{\frac 4 3} - 12 \times 3^{\frac 1 3} + 83, 83 + 16 - 24]$

  $f(x, 2) = x^4+16-8x+2 = x^4 - 8x + 18 \in [2^{\frac 4 3} - 2^{\frac{10}{3}} + 18, 81-24+18]$

  $\therefore $ the absolute maximum value is $83$, and the absolute minimum value is $2$.
  
  \subsection*{37. $f(x, y) = -(x^2-1)^2 - (x^2y -x-1)^2$}

  \begin{proof}

    $f_{x}(x, y) = -4x(x^2-1) -2(x^2y-x-1)(2xy-1)$

    $f_{y}(x, y) = -2x^2(x^2y-x-1)$

    $f_{xx}(x, y) = -4(x^2-1) -8x^2 - 2(2xy-1)^2 -4y(x^2y-x-1)$

    $f_{yy}(x, y) = -2x^2(x^2) = -2x^4$

    $f_{xy}(x, y) = -2(x^2)(2xy-1) -2(x^2y-x-1)(2x)$

    Let $f_x(x, y) = f_y(x, y) = 0$, then $\left\{ \begin{array}{ll} x = 1 \\ y = 2 \end{array}\right.$ or $\left\{ \begin{array}{ll} x = -1 \\ y = 0 \end{array}\right.$

    When $x = 1, y = 2, f_{xx}(x, y) < 0, f_{yy}(x, y) = -2 < 0, f_{xy}(x, y) = -6$

    $D = f_{xx}(x, y)f_{yy}(x, y) - [f_{xy}(x, y)]^2 = 52- 36 > 0$

    $\therefore f$ has a local maximum at $(1, 2)$

    When $x = -1, y = 0, f_{xx}(x, y) = -10 < 0, f_{yy}(x, y) = -2, f_{xy}(x, y) = 2$

    $D = f_{xx}(x, y)f_{yy}(x, y) - [f_{xy}(x, y)]^2 = 20 - 4 > 0$

    $\therefore f$ has a local maximum at $(-1, 0)$

  \end{proof}

  \subsection*{38. }

  \begin{proof}
    $f_x(x, y) = 3e^y - 3x^2 = 3(e^y - x^2)$

    $f_y(x, y) = 3xe^y - 3e^{3y} = 3e^y(x-e^{2y})$

    Let $f_x(x, y) = f_y(x, y) = 0$, then $x = 1, y = 0$

    When $x = 1, y = 0$, $f_{xx}(x, y) = -6 < 0,f_{yy}(x, y) = 3e^y(x-3e^{2y}) = -6 < 0$

    $f_{xy}(x, y) = 3e^y, D = f_{xx}(x, y)f_{yy}(x, y) - [f_{xy}(x, y)]^2 = 36 - 9 > 0$

    $\therefore f$ has a local maximum at $(1, 0)$

    However, $f(-3, 0) = 3(-3) + 27 - 1 = 17 > f(1, 0) = 3 - 1 - 1 = 1$

    $\therefore f(1, 0)$ is not an absolute maximum value

  \end{proof}

  \subsection*{42. }

  Let the coordinate of the point be $(x, y, z)$, then the distance can be expressed as

  $$D = \sqrt{x^2+y^2+z^2} = \sqrt{x^2+z^2+xz + 9}$$

  Let $g(x, y) = x^2+y^2+xy+9$, then find the minimum value of $g(x, y)$

  $g_x(x, y) = 2x + y, g_y(x, y) = 2y + x$

  Let $g_x(x, y) = g_y(x, y) = 0$, then $x = 0, y = 0$

  $g_{xx}(x, y) = 2 > 0, g_{yy}(x, y) = 2, g_{xy}(x, y) = 1, D = 4 - 1 > 0$

  $\therefore g(0, 0) = 9$ is the local minimum value, and absolute minimum value of $g(x, y)$

  $\therefore D_{min} = \sqrt{9} = 3$

  \subsection*{47. }

  Let the coordinate of the vertex be $(x, y, z)$, then the volume can be expressed as 

  $$V = xyz = (6-2y-3z)yz$$

  where $y \geq 0, z \geq 0$.

  Let $g(x, y) = (6-2x-3y)xy$, then find the maximum value of $g(x, y)$

  $g_x(x, y) = -4xy+6y-3y^2, \quad g_y(x, y) = -6xy+6x-2x^2$

  Let $g_x(x, y) = g_y(x, y) = 0$ and $x \not = 0, y \not = 0$, then $x = 1, y = \frac 2 3$

  When $x = 1, y = \frac 2 3$, $g_{xx}(x, y) = -4y = -\frac 8 3 < 0, g_{yy}(x, y) = -6x < 0$

  $g_{xy}(x, y) = -4x+6-6y = -2$

  $D = g_{xx}(x, y)g_{yy}(x, y) - [g_{xy}(x, y)]^2 = 16 - 4 > 0$

  $\therefore g$ attaches its local maximum at $(1, \frac 2 3)$, and $g(1, \frac 2 3) = \frac 4 3$

  If $x = 0$ or $y = 0$, $g(x, y) = 0 < g(1, \frac 2 3)$

  $\therefore g(1, \frac 2 3) = \frac 4 3$ is the absolute maximum of $g(x, y)$

  $\therefore V_{max} = g(1, \frac 2 3) = \frac 4 3$

\end{document}