\documentclass{article}
\usepackage{amsmath}
\usepackage{amsthm}
\usepackage{amssymb}
\usepackage{enumerate}
\usepackage{graphicx}

\begin{document}
  \title{Exercise 14.x}
  \author{Wang Yue from CS Elite Class}
  \date{April 26, 2021}
  \maketitle

  \subsection*{1. (2) $x = a\cos \alpha \cos t, y = a\sin \alpha \cos t, z = a\sin t, t = t_0$}

  $$\because x^2+y^2+z^2 = a^2(\cos^2 \alpha + \sin^2 \alpha) \cos^2 t + a^2 \sin^2 t = a^2$$

  $\therefore$ the curve is a the shell of the sphere, with radius $|a|$.

  Let $\overrightarrow r (t) = \langle a\cos \alpha \cos t, a \sin \alpha \cos t, a \sin t \rangle$, then

  $$\overrightarrow r '(t) = \langle -a \cos \alpha \sin t, -a\sin \alpha \sin t, a \cos t \rangle$$

  $$\therefore \overrightarrow r '(t_0) = \langle -a \cos \alpha \sin t_0, -a\sin \alpha \sin t_0, a \cos t_0 \rangle$$

  \subsection*{1. (4) $z = f(x, y), \frac{x - x_0}{\cos \alpha} = \frac{y - y_0}{\sin \alpha}, f$ is differentiable, $M_0(x_0, y_0, z_0)$}

  Let $z = \varphi (t), \varphi (t) =  f(x_0 + t\cos \alpha,  y_0 + t\sin \alpha)$

  $$\overrightarrow r (t) = \langle
    x_0 + t\cos \alpha, 
    y_0 + t\sin \alpha, 
    f(x_0 + t\cos \alpha, y_0 + t\sin \alpha)
  \rangle $$

  Taking differentiation to $\varphi(t)$ with respect to $t$, we have

  $$\overrightarrow r '(t) = \langle \cos \alpha, \sin \alpha, f_x \cos \alpha + f_y \sin \alpha \rangle$$

  \subsection*{4. }

  Let $F(x, y, z) = x^2+y^2+z^2-3x, G(x, y, z) = 2x - 3y + 5z - 4$, then

  $$\nabla F = \langle 2x-3, 2y, 2z \rangle, \quad \nabla G = \langle 2, -3, 5 \rangle$$

  When $x = 1, y = 1, z = 1, \nabla F = \langle -1, 2, 2 \rangle$

  $\therefore$ the tangent vector at $(1, 1, 1)$ is $$\nabla F \times \nabla G = \langle 16, -9, -1 \rangle$$

  $\therefore$ the equation of the tangent line is $\frac{x-1}{16} = \frac{y-1}{-9} = \frac{z-1}{-1}$.

  $\therefore$ the equation of the normal plane is $16(x-1) -9(y-1) -(z-1) = 0$

  \subsection*{7. (2) $z = e^y + x + x^2 + 6, \quad P_0(1, 0, 9)$}

  Let $f(x, y) = e^y + x + x^2 + 6, F(x, y, z) = f(x, y) - z$, then

  $$f_x(x, y) = 2x + 1, \quad f_y(x, y) = e^y$$

  $$\therefore \nabla F(x, y, z) = \langle 2x + 1, e^y, -1 \rangle$$

  When $x = 1, y = 0, z = 9, \nabla F = \langle 3, 1, -1 \rangle$

  $\therefore$ the equation of the tangent plane at $P_0$ is $3(x-1)+(y-0)-(z-9)=0$

  $\therefore$ the equation of the normal line at $P_0$ is $$\frac{x-1}{3} = \frac{y}{1} = \frac{z-9}{-1}$$

  \subsection*{7. (7) $z = y + \ln \frac x z, \quad P_0(1, 1, 1)$}

  Let $f(x, y) = y + \ln \frac x z, F(x, y, z) = f(x, y) - z$, then

  Let $f(x, y, z) = y + \ln \frac x z - z$, then

  $$f_x = \frac{1}{\frac x z}\frac{1}{z} = \frac 1 x, \quad f_y = 1, \quad f_z = -\frac{1}{\frac x z}\frac{x}{z^2} - 1 = -\frac{1}{z} - 1$$

  $$\therefore \nabla f(x, y, z) = \langle \frac 1 x, 1, -\frac 1 z - 1 \rangle$$

  When $x = 1, y = 1, z = 1$, $\nabla f = \langle 1, 1, -2 \rangle$

  $\therefore$ the equation of the tangent plane at $P_0$ is $(x - 1) + (y-1) -2(z-1) = 0$

  $\therefore$ the equation of the normal line at $P_0$ is

  $$\frac{x-1}{1} = \frac{y-1}{1} = \frac{z-1}{-2}$$

  \subsection*{8. }

  Let $F(x, y, z) = 2x^2+3y^2+z^2-9$, then $F_x = 4x, F_y = 6y, F_z = 2z$

  $$\therefore \nabla F(x, y, z) = \langle 4x, 6y, 2z \rangle$$

  Let $\overrightarrow n = \langle 2, -3, 2 \rangle$, and let $\nabla F \parallel \overrightarrow n$, then we have

  $$\frac{4x}{2} = \frac{6y}{-3} = \frac{2z}{2}$$

  $$\therefore y = -x, z = 2x$$

  $\therefore 2x^2 + 3x^2+4x^2 = 9x^2 = 9$, then $x = \pm 1$

  $\therefore$ the normal vector is $(4, -6, 4)$ or $(-4, 6, -4)$

  $\therefore$ the equation of the tangent plane is $$4(x-1)-6(y+1)+4(z-2) = 0 \textrm{ or } -4(x-1)+6(y+1)-4(z-2) = 0$$

  $$\textrm{i.e. } 2x-3y+2z=\pm 9$$

  \section*{B}

  \subsection*{1. }

  \begin{proof}
    Let $\overrightarrow{r} (t) = \left\{ \begin{array}{ll} x = ae^t \cos t \\ y = ae^t \sin t \\ z = ae^t \end{array}\right.$, then
    $\overrightarrow{r'}(t) = \left\{ \begin{array}{ll} x = ae^t(\cos t - \sin t) \\ y = ae^t(\sin t + \cos t) \\ z = ae^t\end{array} \right.$

    The direction vector of generatrix is $\overrightarrow{s}(t) = \left\{ \begin{array}{ll} x = ae^{t} \cos t \\ y = ae^t \sin t \\ z = ae^t \end{array} \right.$

    Let $\theta$ be the angle between $\overrightarrow r$ and $\overrightarrow s$, then

    $$\cos \theta = \frac{\overrightarrow r \cdot \overrightarrow s}{|\overrightarrow r| |\overrightarrow s|} = \frac{\sqrt 6}{3}$$

    $\therefore \theta$ is a constant
      
  \end{proof}

  \subsection*{3. }

  Let $\overrightarrow{n_1} = (1, -1, -1), \overrightarrow{n_2} = (1, -1, -\frac 1 2)$, then

  $$\overrightarrow{n} = \overrightarrow{n_1} \times \overrightarrow{n_2} = (-\frac 1 2, \frac 1 2, 0)$$

  Let $F(x, y, z) = x^2+y^2+z^2-x$, then

  $$F_x = 2x-1, \quad F_y = 2y, \quad F_z = 2z$$

  $$\therefore \nabla F(x, y, z) = \langle 2x-1, 2y, 2z \rangle$$

  $$\therefore y=-x+\frac 1 2, \quad z = 0$$

  $$\therefore F(x, y, z) = x^2 + x^2 + \frac 1 4 - x + 0 - x = 0$$

  $$\therefore x = \frac{1\pm \frac{\sqrt 2}{2}}{2} = \frac{2 \pm \sqrt 2}{4}, y = \frac{\pm \sqrt 2}{4}, z = 0$$

  $\therefore$ the equation of the tangent plane is $$x + y = \frac{1 \pm \sqrt 2}{2}$$



\end{document}