\documentclass{article}
\usepackage{amsmath}
\usepackage{amsthm}
\usepackage{amssymb}
\usepackage{enumerate}
\usepackage{graphicx}

\begin{document}
  \title{Exercise 14.8}
  \author{Wang Yue from CS Elite Class}
  \date{\today}
  \maketitle

  \subsection*{1. Find the point on the curve of intersection of the paraboloid $z = x^2+y^2$ and the plane $x+y+2z=2$ that are closest and farthest from the origin.}

  Let the distance between a point to the origin be $d = \sqrt{x^2+y^2+z^2}$, then for convenience we solve the maximum and minimum of $d^2$ under constraints.

  Construct the Lagrange Function $$L(x, y, z, \lambda, \mu) = (x^2+y^2+z^2) + \lambda (x^2+y^2-z^2) + \mu(x+y+2z-2)$$
  
  then let $$\left\{ \begin{array}{ll} 
    \frac{\partial L}{\partial x} = 2x + 2 \lambda x + \mu &= 0 \\
    \frac{\partial L}{\partial y} = 2y + 2 \lambda y + \mu &= 0 \\
    \frac{\partial L}{\partial z} = 2z + 2 \lambda z + 2 \mu &= 0 \\
    \frac{\partial L}{\partial \lambda} = x^2 = y^2 - z^2 &= 0 \\
    \frac{\partial L}{\partial \mu} = x + y + 2z - 2 &= 0
  \end{array}\right.$$

  then we can get $\left\{ \begin{array}{ll} x = \frac 1 2 \\ y = \frac 1 2 \\ z = -\frac 1 2 \end{array}\right.$ or $\left\{ \begin{array}{ll} x = -1 \\ y = -1 \\ z = 2 \end{array}\right.$

  When $x = y = \frac 1 2, z = -\frac 1 2$, $d = \sqrt{3 \times \frac 1 4} = \frac{\sqrt 3}{2}$

  When $x = y = -1, z = 2$, $d = \sqrt{1 + 1 + 4} = \sqrt 6$

  $\therefore$ the closet distance is $\frac{\sqrt 3}{2}$, and the farthest distance is $\sqrt 6$.

  \subsection*{2. }

  Let $F(x, y, z) = \frac{x^2}{a^2} + \frac{y^2}{b^2} + \frac{z^2}{c^2} - 1$, then $\nabla F = \langle \frac{2x}{a^2}, \frac{2y}{b^2}, \frac{2z}{c^2} \rangle$

  $\therefore$ the equation of the tangent plane is $$\frac{2x_0}{a^2}(x-x_0) + \frac{2y_0}{b^2}(y-y_0) + \frac{2z_0}{c^2}(z-z_0)$$

  Let $x = y = 0$, then we get the intercept in z-axis, i.e. $$z = (\frac{2x_0^2}{a^2} + \frac{2y_0^2}{b^2} + \frac{2z_0^2}{c^2}) \times \frac{c^2}{2z_0} = \frac{c^2}{z_0}$$

  And similarly, we can get the intercept $y = \frac{b^2}{y_0}$ in y-axis and $x = \frac{a^2}{x_0}$ in x-axis.

  $\therefore$ the volume of the tetrahedron, i.e $$V = \frac 1 3 (\frac 1 2 \frac{a^2}{x_0} \frac{b^2}{y_0}) \frac{c^2}{z_0} = \frac{a^2b^2c^2}{6x_0y_0z_0}$$

  Construct Lagrange Function $L(x, y, z, \lambda) = \frac{a^2b^2c^2}{6xyz} + \lambda (\frac{x^2}{a^2} + \frac{y^2}{b^2} + \frac{z^2}{c^2} - 1) = 0$, then let

  $$\left\{ \begin{array}{ll} 
    \frac{\partial L}{\partial x} = -\frac{a^2b^2c^2}{6x^2yz} + \frac{2x\lambda}{a^2} = 0 \\
    \frac{\partial L}{\partial y} = -\frac{a^2b^2c^2}{6xy^2z} + \frac{2y\lambda}{b^2} = 0 \\
    \frac{\partial L}{\partial z} = -\frac{a^2b^2c^2}{6xyz^2} + \frac{2z\lambda}{c^2} = 0 \\
    \frac{\partial L}{\partial \lambda} = \frac{x^2}{a^2} + \frac{y^2}{b^2} + \frac{z^2}{c^2} - 1 = 0
  \end{array}\right.$$

  From $\frac{\partial L}{\partial x} = \frac{\partial L}{\partial y} = \frac{\partial L}{\partial z} = 0$, we can get $$\frac{x^2}{a^2} = \frac{y^2}{b^2} = \frac{z^2}{c^2} = \frac{a^2b^2c^2}{12xyz\lambda}$$

  $\therefore$ $\frac{x^2}{a^2} = \frac{y^2}{b^2} = \frac{z^2}{c^2} = \frac 1 3$, which means $x = \frac{a}{\sqrt 3}, y = \frac{b}{\sqrt 3}, z = \frac{c}{\sqrt 3}$

  $\therefore$ we have the minimum of volume $V_{min} = \frac{\sqrt 3abc}{2}$

  \subsection*{3. }

  Construct Lagrange Function $$L(x, y, z, \lambda) = x^2 + \pi y^2 + \frac{\sqrt 3z^2}{4} + \lambda (4x + 2\pi y + 3z - 2m)$$

  then let

  $$\left\{ \begin{array}{ll} 
    \frac{\partial L}{\partial x} = 2x + 4\lambda = 0 \\
    \frac{\partial L}{\partial y} = 2\pi y + 2\pi\lambda = 0 \\
    \frac{\partial L}{\partial z} = \frac{\sqrt 3 z}{2} + 3\lambda = 0 \\
    \frac{\partial L}{\partial \lambda} = 4x + 2\pi y + 3z - 2m = 0
  \end{array}\right.$$

  we get $$\left\{\begin{array}{ll}  x = -2\lambda \\ y = -\lambda \\ z = -2 \sqrt 3 \lambda\end{array}\right.$$

  then $-8\lambda - 2\pi \lambda - 6\sqrt 3 \lambda = 2m$, i.e.

  $$\lambda = -\frac{m}{4 + \pi + 3\sqrt 3}$$

  $\therefore x = \frac{2m}{4 + \pi + 3\sqrt 3}, y = \frac{m}{4 + \pi + 3\sqrt 3}, z = \frac{2\sqrt 3 m}{4 + \pi + 3\sqrt 3}$

  $\therefore$ the maximum sum of area is $$x^2 + \pi y^2 + \frac{\sqrt 3 z^2}{4} = \frac{4m^2 + \pi m^2 + 3\sqrt 3m^2}{(4 + \pi + 3\sqrt 3)^2} = \frac{m^2}{4+\pi+3\sqrt 3}$$

  \subsection*{4. }

  $f(x, y) = x^2y(4-x-y)$

  $D = \{ (x, y) | x + y \leq 6 \textrm{ and } x \geq 0 \textrm{ and } y \geq 0 \}$

  $f_x(x, y) = y[2x(4-x-y) - x^2] = 8xy - 3x^2y -2xy^2$

  $f_y(x, y) = x^2[(4-x-y) -1] = 3x^2-x^3-x^2y$

  Let $f_x(x, y) = f_y(x, y) = 0$ and do not consider boundary, we get $x = 2, y = 1$

  $f_{xx}(x, y) = 8y - 6xy - 2y^2$
  
  $f_{yy}(x, y) = -x^2$

  $f_{xy}(x, y) = 8x - 3x^2 - 4xy$

  $$\begin{aligned}
    D &= f_{xx}f_{yy} - (f_{xy})^2 \\
    &= -8x^2y + 6x^3y + 2x^2y^2 - (64x^2 + 9x^4 + 16x^2y^2 - 48x^3 - 64x^2y + 24x^3y) \\
    &= 56x^2y - 18x^3y - 14x^2y^2 - 64x^2 - 9x^4 + 48x^3
  \end{aligned}$$

  When $x = 2, y = 1$, $D = 56 \times 4 - 18 \times 8 - 14 \times 4 - 64 \times 4 - 9 \times 16 + 48 \times 8 = 8 > 0$

  $\because f_{xx}(2, 1) = 8 - 12 - 2 = -2 < 0$

  $\therefore f(2, 1) = 4\times 1 \times (4-2-1) = 4$ is a local maximum

  Fix $x = 0, 0 \leq y \leq 6$, then $f(0, y) = 0$

  Fix $y = 0, 0 \leq x \leq 6$, then $f(x, 0) = 0$

  Fix $x + y = 6$, then $f(x, y) = x^2(6-x)(4-6) = 2x^3 - 12x^2$, where $0 \leq x \leq 6$

  Let $g(x) = 2x^3 - 12x^2$, then $g'(x) = 6x^2 - 24x = 6x(x - 4)$

  When $x = 0, g(x) = 0$. When $x = 4, g(x) = 128 - 12 \times 16 = -64$

  $\therefore f(2, 1) = 4$ is a local maximum, and there is no local minimum

  $\therefore f(2, 1) = 4$ is the absolute maximum, and $f(4, 2) = -64$ is the absolute minimum.

\end{document}