\documentclass{article}
\usepackage{amsmath}
\usepackage{amsthm}
\usepackage{amssymb}
\usepackage{enumerate}
\usepackage{graphicx}

\begin{document}
    \title{Homework}
    \date{\today}
    \maketitle

    $\because \left\{ \begin{array}{ll} x = 3 \cos t \\ y = 2\sin t \end{array}\right.$

    $\therefore r(t) = (3\cos t, 2\sin t, 0)$

    $$\therefore r'(t) = (-3\sin t, 2\cos t, 0), r''(t) = (-3\cos t, -2\sin t, 0)$$

    $$\therefore r'(t) \times r''(t) = (0, 0, 6\sin^2 t + 6\cos^2 t) = (0, 0, 6)$$
{
    $$\therefore k = \frac{|r'(t) \times r''(t)|}{|r'(t)|^3} = \frac{6}{(\sqrt{9\sin^2 t + 4\cos^2 t})^3}$$

    $\therefore$ When $t = 0$, $k = \frac{6}{\sqrt{4}^3} = \frac{3}{4}$

    $\therefore$ When $t = \frac \pi 2$, $k = \frac{6}{\sqrt{9}^3} = \frac{2}{9}$

    $\because$ Generally, for a circle $x^2 + y^2 = R^2$, we have:

    $$r(t) = (R\cos t, R\sin t, 0)$$

    $\therefore r'(t) = (-R\sin t, R\cos t, 0), r''(t) = (-R\cos t, -R\sin t, 0)$

    $$\therefore k = \frac{|r'(t) \times r''(t)|}{|r'(t)|^3} = \frac{R^2}{R^3} = \frac{1}{R}$$

    $\therefore$ When $t = 0$, $r(t) = (3, 0, 0)$, the corresponding circle of curvature has radius $\frac{1}{k} = \frac 4 3$, and the center is at $(\frac 5 3, 0)$, which satisfies the equation: $$(x - \frac 5 3)^2 + y^2 = \frac{16}{9}$$

    $\therefore$ When $t = \frac \pi 2$, $r(t) = (0, 2, 0)$, the corresponding circle of curvature has radius $\frac 1 k = \frac 9 2$, and the center is at $(0, -\frac 5 2)$, which satisfies the equation: $$x^2 + (y + \frac 5 2)^2 = \frac{81}{4}$$

\end{document}